lava/out/Benchmark/PeanoNats.v
@@ -36,7 +36,7 @@ Qed.
 Fixpoint Nats_wf (x : Nats_u): Prop :=
   match x with | Suc_u n => Nats_wf n ∧ True | Zero_u => True end.
 
-Theorem Nats_wf_ref [p : Nats_u → Prop] (tm : {v: Nats_u | Nats_wf v ∧ p v}): Nats_wf ⌊ tm ⌋.
+Theorem Nats_wf_ref [p : Nats_u → Prop] (tm : {v: Nats_u | Nats_wf v ∧ p v}): Nats_wf ⌊ tm -⌋.
 Proof.
   destruct tm as [tm tm_p]. solver.
 Qed.
@@ -126,12 +126,15 @@ Qed.
 #[global] Hint Rewrite add_Suc_x_lem: f_rel_back.
 
 Theorem add_rel_ex (m : Nats_u) (m_p : Nats_wf m ∧ True) (n : Nats_u) (n_p : Nats_wf n ∧ True):
-  add_rel m n ⌊ add (exist _ m m_p) (exist _ n n_p) ⌋.
+  add_rel m n ⌊ add (exist _ m m_p) (exist _ n n_p) -⌋.
 Proof.
   Opaque add.
   existence_lemma_pre add;
   try revert n_p; generalize dependent n; induction m as [m IH_m|]; intros;
-  [fix_notations | fix_notations];
+  [fix_notations;
+   pose proof (IH_m ltac:(try clear IH_m; solver) n ltac:(try clear IH_m; solver)) as IH_14792487;
+   try clear IH_m |
+   fix_notations];
   simpl in *.
   Transparent add.
   all: existence_lemma_quicksolve add; f__f_rel_ex_body; f_rel_finish.
@@ -143,7 +146,7 @@ Qed.
 
 Theorem add__add_rel_rw
   (m : Nats_u) (m_p : Nats_wf m ∧ True) (n : Nats_u) (n_p : Nats_wf n ∧ True) (VV : Nats_u):
-  ⌊ add (exist _ m m_p) (exist _ n n_p) ⌋ = VV ↔ add_rel m n VV.
+  ⌊ add (exist _ m m_p) (exist _ n n_p) -⌋ = VV ↔ add_rel m n VV.
 Proof.
   f__f_rel_rw.
 Qed.
@@ -154,7 +157,7 @@ Qed.
 
 #[global] Instance add_lookup_rw: dictionary rwLem add := { lookup' := add__add_rel_rw }.
 
-Theorem add__add_rel (m n : Nats) (VV : Nats_u): ⌊ add m n ⌋ = VV ↔ add_rel ⌊ m ⌋ ⌊ n ⌋ VV.
+Theorem add__add_rel (m n : Nats) (VV : Nats_u): ⌊ add m n -⌋ = VV ↔ add_rel ⌊ m ⌋ ⌊ n ⌋ VV.
 Proof.
   f__f_rel.
 Qed.
@@ -162,7 +165,7 @@ Qed.
 #[global] Hint Rewrite add__add_rel: f_rel_funct_db.
 
 Theorem add__add_rel' (m_u n_u : Nats_u) (m n : Nats) (VV : Nats_u):
-  m_u = ⌊ m ⌋ → (n_u = ⌊ n ⌋ → ⌊ add m n ⌋ = VV ↔ add_rel m_u n_u VV).
+  m_u = ⌊ m ⌋ → (n_u = ⌊ n ⌋ → ⌊ add m n -⌋ = VV ↔ add_rel m_u n_u VV).
 Proof.
   intros -> ->. refine (add__add_rel m n VV).
 Qed.
@@ -448,7 +451,7 @@ Qed.
 #[global] Hint Rewrite eqN_Suc_Suc_lem: f_rel_back.
 
 Theorem eqN_rel_ex (m : Nats_u) (m_p : Nats_wf m ∧ True) (n : Nats_u) (n_p : Nats_wf n ∧ True):
-  eqN_rel m n ⌊ eqN (exist _ m m_p) (exist _ n n_p) ⌋.
+  eqN_rel m n ⌊ eqN (exist _ m m_p) (exist _ n n_p) -⌋.
 Proof.
   Opaque eqN.
   existence_lemma_pre eqN;
@@ -471,7 +474,7 @@ Qed.
 
 Theorem eqN__eqN_rel_rw
   (m : Nats_u) (m_p : Nats_wf m ∧ True) (n : Nats_u) (n_p : Nats_wf n ∧ True) (VV : bool):
-  ⌊ eqN (exist _ m m_p) (exist _ n n_p) ⌋ = VV ↔ eqN_rel m n VV.
+  ⌊ eqN (exist _ m m_p) (exist _ n n_p) -⌋ = VV ↔ eqN_rel m n VV.
 Proof.
   f__f_rel_rw.
 Qed.
@@ -482,7 +485,7 @@ Qed.
 
 #[global] Instance eqN_lookup_rw: dictionary rwLem eqN := { lookup' := eqN__eqN_rel_rw }.
 
-Theorem eqN__eqN_rel (m n : Nats) (VV : bool): ⌊ eqN m n ⌋ = VV ↔ eqN_rel ⌊ m ⌋ ⌊ n ⌋ VV.
+Theorem eqN__eqN_rel (m n : Nats) (VV : bool): ⌊ eqN m n -⌋ = VV ↔ eqN_rel ⌊ m ⌋ ⌊ n ⌋ VV.
 Proof.
   f__f_rel.
 Qed.
@@ -490,7 +493,7 @@ Qed.
 #[global] Hint Rewrite eqN__eqN_rel: f_rel_funct_db.
 
 Theorem eqN__eqN_rel' (m_u n_u : Nats_u) (m n : Nats) (VV : bool):
-  m_u = ⌊ m ⌋ → (n_u = ⌊ n ⌋ → ⌊ eqN m n ⌋ = VV ↔ eqN_rel m_u n_u VV).
+  m_u = ⌊ m ⌋ → (n_u = ⌊ n ⌋ → ⌊ eqN m n -⌋ = VV ↔ eqN_rel m_u n_u VV).
 Proof.
   intros -> ->. refine (eqN__eqN_rel m n VV).
 Qed.
@@ -628,7 +631,7 @@ Qed.
 #[global] Hint Rewrite geqN_Suc_Suc_lem: f_rel_back.
 
 Theorem geqN_rel_ex (m : Nats_u) (m_p : Nats_wf m ∧ True) (n : Nats_u) (n_p : Nats_wf n ∧ True):
-  geqN_rel m n ⌊ geqN (exist _ m m_p) (exist _ n n_p) ⌋.
+  geqN_rel m n ⌊ geqN (exist _ m m_p) (exist _ n n_p) -⌋.
 Proof.
   Opaque geqN.
   existence_lemma_pre geqN;
@@ -655,7 +658,7 @@ Qed.
 
 Theorem geqN__geqN_rel_rw
   (m : Nats_u) (m_p : Nats_wf m ∧ True) (n : Nats_u) (n_p : Nats_wf n ∧ True) (VV : bool):
-  ⌊ geqN (exist _ m m_p) (exist _ n n_p) ⌋ = VV ↔ geqN_rel m n VV.
+  ⌊ geqN (exist _ m m_p) (exist _ n n_p) -⌋ = VV ↔ geqN_rel m n VV.
 Proof.
   f__f_rel_rw.
 Qed.
@@ -666,7 +669,7 @@ Qed.
 
 #[global] Instance geqN_lookup_rw: dictionary rwLem geqN := { lookup' := geqN__geqN_rel_rw }.
 
-Theorem geqN__geqN_rel (m n : Nats) (VV : bool): ⌊ geqN m n ⌋ = VV ↔ geqN_rel ⌊ m ⌋ ⌊ n ⌋ VV.
+Theorem geqN__geqN_rel (m n : Nats) (VV : bool): ⌊ geqN m n -⌋ = VV ↔ geqN_rel ⌊ m ⌋ ⌊ n ⌋ VV.
 Proof.
   f__f_rel.
 Qed.
@@ -674,7 +677,7 @@ Qed.
 #[global] Hint Rewrite geqN__geqN_rel: f_rel_funct_db.
 
 Theorem geqN__geqN_rel' (m_u n_u : Nats_u) (m n : Nats) (VV : bool):
-  m_u = ⌊ m ⌋ → (n_u = ⌊ n ⌋ → ⌊ geqN m n ⌋ = VV ↔ geqN_rel m_u n_u VV).
+  m_u = ⌊ m ⌋ → (n_u = ⌊ n ⌋ → ⌊ geqN m n -⌋ = VV ↔ geqN_rel m_u n_u VV).
 Proof.
   intros -> ->. refine (geqN__geqN_rel m n VV).
 Qed.
@@ -764,12 +767,15 @@ Qed.
 #[global] Hint Rewrite mult_Suc_x_lem: f_rel_back.
 
 Theorem mult_rel_ex (m : Nats_u) (m_p : Nats_wf m ∧ True) (n : Nats_u) (n_p : Nats_wf n ∧ True):
-  mult_rel m n ⌊ mult (exist _ m m_p) (exist _ n n_p) ⌋.
+  mult_rel m n ⌊ mult (exist _ m m_p) (exist _ n n_p) -⌋.
 Proof.
   Opaque mult.
   existence_lemma_pre mult;
   try revert n_p; generalize dependent n; induction m as [m IH_m|]; intros;
-  [fix_notations | fix_notations];
+  [fix_notations;
+   pose proof (IH_m ltac:(try clear IH_m; solver) n ltac:(try clear IH_m; solver)) as IH_14792487;
+   try clear IH_m |
+   fix_notations];
   simpl in *.
   Transparent mult.
   all: existence_lemma_quicksolve mult; f__f_rel_ex_body; f_rel_finish.
@@ -781,7 +787,7 @@ Qed.
 
 Theorem mult__mult_rel_rw
   (m : Nats_u) (m_p : Nats_wf m ∧ True) (n : Nats_u) (n_p : Nats_wf n ∧ True) (VV : Nats_u):
-  ⌊ mult (exist _ m m_p) (exist _ n n_p) ⌋ = VV ↔ mult_rel m n VV.
+  ⌊ mult (exist _ m m_p) (exist _ n n_p) -⌋ = VV ↔ mult_rel m n VV.
 Proof.
   f__f_rel_rw.
 Qed.
@@ -792,7 +798,7 @@ Qed.
 
 #[global] Instance mult_lookup_rw: dictionary rwLem mult := { lookup' := mult__mult_rel_rw }.
 
-Theorem mult__mult_rel (m n : Nats) (VV : Nats_u): ⌊ mult m n ⌋ = VV ↔ mult_rel ⌊ m ⌋ ⌊ n ⌋ VV.
+Theorem mult__mult_rel (m n : Nats) (VV : Nats_u): ⌊ mult m n -⌋ = VV ↔ mult_rel ⌊ m ⌋ ⌊ n ⌋ VV.
 Proof.
   f__f_rel.
 Qed.
@@ -800,7 +806,7 @@ Qed.
 #[global] Hint Rewrite mult__mult_rel: f_rel_funct_db.
 
 Theorem mult__mult_rel' (m_u n_u : Nats_u) (m n : Nats) (VV : Nats_u):
-  m_u = ⌊ m ⌋ → (n_u = ⌊ n ⌋ → ⌊ mult m n ⌋ = VV ↔ mult_rel m_u n_u VV).
+  m_u = ⌊ m ⌋ → (n_u = ⌊ n ⌋ → ⌊ mult m n -⌋ = VV ↔ mult_rel m_u n_u VV).
 Proof.
   intros -> ->. refine (mult__mult_rel m n VV).
 Qed.
@@ -954,7 +960,7 @@ Qed.
 
 #[global] Hint Rewrite one_inv_lem: f_rel_back.
 
-Theorem one_rel_ex : one_rel ⌊ one ⌋.
+Theorem one_rel_ex : one_rel ⌊ one -⌋.
 Proof.
   Opaque one.
   existence_lemma_pre one; fix_notations; simpl in *.
@@ -966,7 +972,7 @@ Qed.
 
 #[global] Opaque one.
 
-Theorem one__one_rel_rw (VV : Nats_u): ⌊ one ⌋ = VV ↔ one_rel VV.
+Theorem one__one_rel_rw (VV : Nats_u): ⌊ one -⌋ = VV ↔ one_rel VV.
 Proof.
   f__f_rel_rw.
 Qed.
@@ -977,14 +983,14 @@ Qed.
 
 #[global] Instance one_lookup_rw: dictionary rwLem one := { lookup' := one__one_rel_rw }.
 
-Theorem one__one_rel (VV : Nats_u): ⌊ one ⌋ = VV ↔ one_rel VV.
+Theorem one__one_rel (VV : Nats_u): ⌊ one -⌋ = VV ↔ one_rel VV.
 Proof.
   f__f_rel.
 Qed.
 
 #[global] Hint Rewrite one__one_rel: f_rel_funct_db.
 
-Theorem one__one_rel' (VV : Nats_u): ⌊ one ⌋ = VV ↔ one_rel VV.
+Theorem one__one_rel' (VV : Nats_u): ⌊ one -⌋ = VV ↔ one_rel VV.
 Proof.
   intros. refine (one__one_rel VV).
 Qed.
@@ -1082,7 +1088,7 @@ Theorem sub_rel_ex
   (m_p : Nats_wf m ∧ True)
   (n : Nats_u)
   (n_p : Nats_wf n ∧ ∃ geqN_res, geqN_rel m n geqN_res ∧ is_true geqN_res):
-  sub_rel m n ⌊ sub (exist _ m m_p) (exist _ n n_p) ⌋.
+  sub_rel m n ⌊ sub (exist _ m m_p) (exist _ n n_p) -⌋.
 Proof.
   Opaque sub.
   existence_lemma_pre sub;
@@ -1109,7 +1115,7 @@ Theorem sub__sub_rel_rw
   (n : Nats_u)
   (n_p : Nats_wf n ∧ ∃ geqN_res, geqN_rel m n geqN_res ∧ is_true geqN_res)
   (o : Nats_u):
-  ⌊ sub (exist _ m m_p) (exist _ n n_p) ⌋ = o ↔ sub_rel m n o.
+  ⌊ sub (exist _ m m_p) (exist _ n n_p) -⌋ = o ↔ sub_rel m n o.
 Proof.
   f__f_rel_rw.
 Qed.
@@ -1124,7 +1130,7 @@ Theorem sub__sub_rel
   (m : Nats)
   (n : {n: Nats_u | Nats_wf n ∧ ∃ geqN_res, geqN_rel ⌊ m ⌋ n geqN_res ∧ is_true geqN_res})
   (o : Nats_u):
-  ⌊ sub m n ⌋ = o ↔ sub_rel ⌊ m ⌋ ⌊ n ⌋ o.
+  ⌊ sub m n -⌋ = o ↔ sub_rel ⌊ m ⌋ ⌊ n ⌋ o.
 Proof.
   f__f_rel.
 Qed.
@@ -1136,7 +1142,7 @@ Theorem sub__sub_rel'
   (m : Nats)
   (n : {n: Nats_u | Nats_wf n ∧ ∃ geqN_res, geqN_rel ⌊ m ⌋ n geqN_res ∧ is_true geqN_res})
   (o : Nats_u):
-  m_u = ⌊ m ⌋ → (n_u = ⌊ n ⌋ → ⌊ sub m n ⌋ = o ↔ sub_rel m_u n_u o).
+  m_u = ⌊ m ⌋ → (n_u = ⌊ n ⌋ → ⌊ sub m n -⌋ = o ↔ sub_rel m_u n_u o).
 Proof.
   intros -> ->. refine (sub__sub_rel m n o).
 Qed.
@@ -1317,7 +1323,7 @@ Qed.
 
 #[global] Hint Rewrite two_inv_lem: f_rel_back.
 
-Theorem two_rel_ex : two_rel ⌊ two ⌋.
+Theorem two_rel_ex : two_rel ⌊ two -⌋.
 Proof.
   Opaque two.
   existence_lemma_pre two; fix_notations; simpl in *.
@@ -1329,7 +1335,7 @@ Qed.
 
 #[global] Opaque two.
 
-Theorem two__two_rel_rw (VV : Nats_u): ⌊ two ⌋ = VV ↔ two_rel VV.
+Theorem two__two_rel_rw (VV : Nats_u): ⌊ two -⌋ = VV ↔ two_rel VV.
 Proof.
   f__f_rel_rw.
 Qed.
@@ -1340,14 +1346,14 @@ Qed.
 
 #[global] Instance two_lookup_rw: dictionary rwLem two := { lookup' := two__two_rel_rw }.
 
-Theorem two__two_rel (VV : Nats_u): ⌊ two ⌋ = VV ↔ two_rel VV.
+Theorem two__two_rel (VV : Nats_u): ⌊ two -⌋ = VV ↔ two_rel VV.
 Proof.
   f__f_rel.
 Qed.
 
 #[global] Hint Rewrite two__two_rel: f_rel_funct_db.
 
-Theorem two__two_rel' (VV : Nats_u): ⌊ two ⌋ = VV ↔ two_rel VV.
+Theorem two__two_rel' (VV : Nats_u): ⌊ two -⌋ = VV ↔ two_rel VV.
 Proof.
   intros. refine (two__two_rel VV).
 Qed.
