lava/out/Benchmark/SoftwareFoundationsBasics.v
@@ -11,7 +11,7 @@ Fixpoint SFBool_wf (x : SFBool_u): Prop :=
   match x with | SFFalse_u => True | SFTrue_u => True end.
 
 Theorem SFBool_wf_ref [p : SFBool_u → Prop] (tm : {v: SFBool_u | SFBool_wf v ∧ p v}):
-  SFBool_wf ⌊ tm ⌋.
+  SFBool_wf ⌊ tm -⌋.
 Proof.
   destruct tm as [tm tm_p]. solver.
 Qed.
@@ -94,7 +94,7 @@ Qed.
 
 Theorem andb_rel_ex
   (b1 : SFBool_u) (b1_p : SFBool_wf b1 ∧ True) (b2 : SFBool_u) (b2_p : SFBool_wf b2 ∧ True):
-  andb_rel b1 b2 ⌊ andb (exist _ b1 b1_p) (exist _ b2 b2_p) ⌋.
+  andb_rel b1 b2 ⌊ andb (exist _ b1 b1_p) (exist _ b2 b2_p) -⌋.
 Proof.
   Opaque andb.
   existence_lemma_pre andb;
@@ -115,7 +115,7 @@ Theorem andb__andb_rel_rw
   (b2 : SFBool_u)
   (b2_p : SFBool_wf b2 ∧ True)
   (VV : SFBool_u):
-  ⌊ andb (exist _ b1 b1_p) (exist _ b2 b2_p) ⌋ = VV ↔ andb_rel b1 b2 VV.
+  ⌊ andb (exist _ b1 b1_p) (exist _ b2 b2_p) -⌋ = VV ↔ andb_rel b1 b2 VV.
 Proof.
   f__f_rel_rw.
 Qed.
@@ -127,7 +127,7 @@ Qed.
 #[global] Instance andb_lookup_rw: dictionary rwLem andb := { lookup' := andb__andb_rel_rw }.
 
 Theorem andb__andb_rel (b1 b2 : SFBool) (VV : SFBool_u):
-  ⌊ andb b1 b2 ⌋ = VV ↔ andb_rel ⌊ b1 ⌋ ⌊ b2 ⌋ VV.
+  ⌊ andb b1 b2 -⌋ = VV ↔ andb_rel ⌊ b1 ⌋ ⌊ b2 ⌋ VV.
 Proof.
   f__f_rel.
 Qed.
@@ -135,7 +135,7 @@ Qed.
 #[global] Hint Rewrite andb__andb_rel: f_rel_funct_db.
 
 Theorem andb__andb_rel' (b1_u b2_u : SFBool_u) (b1 b2 : SFBool) (VV : SFBool_u):
-  b1_u = ⌊ b1 ⌋ → (b2_u = ⌊ b2 ⌋ → ⌊ andb b1 b2 ⌋ = VV ↔ andb_rel b1_u b2_u VV).
+  b1_u = ⌊ b1 ⌋ → (b2_u = ⌊ b2 ⌋ → ⌊ andb b1 b2 -⌋ = VV ↔ andb_rel b1_u b2_u VV).
 Proof.
   intros -> ->. refine (andb__andb_rel b1 b2 VV).
 Qed.
@@ -270,7 +270,7 @@ Theorem andb3_rel_ex
   (b2_p : SFBool_wf b2 ∧ True)
   (b3 : SFBool_u)
   (b3_p : SFBool_wf b3 ∧ True):
-  andb3_rel b1 b2 b3 ⌊ andb3 (exist _ b1 b1_p) (exist _ b2 b2_p) (exist _ b3 b3_p) ⌋.
+  andb3_rel b1 b2 b3 ⌊ andb3 (exist _ b1 b1_p) (exist _ b2 b2_p) (exist _ b3 b3_p) -⌋.
 Proof.
   Opaque andb3.
   existence_lemma_pre andb3;
@@ -297,7 +297,7 @@ Theorem andb3__andb3_rel_rw
   (b3 : SFBool_u)
   (b3_p : SFBool_wf b3 ∧ True)
   (VV : SFBool_u):
-  ⌊ andb3 (exist _ b1 b1_p) (exist _ b2 b2_p) (exist _ b3 b3_p) ⌋ = VV ↔ andb3_rel b1 b2 b3 VV.
+  ⌊ andb3 (exist _ b1 b1_p) (exist _ b2 b2_p) (exist _ b3 b3_p) -⌋ = VV ↔ andb3_rel b1 b2 b3 VV.
 Proof.
   f__f_rel_rw.
 Qed.
@@ -309,7 +309,7 @@ Qed.
 #[global] Instance andb3_lookup_rw: dictionary rwLem andb3 := { lookup' := andb3__andb3_rel_rw }.
 
 Theorem andb3__andb3_rel (b1 b2 b3 : SFBool) (VV : SFBool_u):
-  ⌊ andb3 b1 b2 b3 ⌋ = VV ↔ andb3_rel ⌊ b1 ⌋ ⌊ b2 ⌋ ⌊ b3 ⌋ VV.
+  ⌊ andb3 b1 b2 b3 -⌋ = VV ↔ andb3_rel ⌊ b1 ⌋ ⌊ b2 ⌋ ⌊ b3 ⌋ VV.
 Proof.
   f__f_rel.
 Qed.
@@ -318,7 +318,7 @@ Qed.
 
 Theorem andb3__andb3_rel' (b1_u b2_u b3_u : SFBool_u) (b1 b2 b3 : SFBool) (VV : SFBool_u):
   b1_u = ⌊ b1 ⌋
-  → (b2_u = ⌊ b2 ⌋ → (b3_u = ⌊ b3 ⌋ → ⌊ andb3 b1 b2 b3 ⌋ = VV ↔ andb3_rel b1_u b2_u b3_u VV)).
+  → (b2_u = ⌊ b2 ⌋ → (b3_u = ⌊ b3 ⌋ → ⌊ andb3 b1 b2 b3 -⌋ = VV ↔ andb3_rel b1_u b2_u b3_u VV)).
 Proof.
   intros -> -> ->. refine (andb3__andb3_rel b1 b2 b3 VV).
 Qed.
@@ -635,7 +635,7 @@ Qed.
 
 Theorem nandb_rel_ex
   (b1 : SFBool_u) (b1_p : SFBool_wf b1 ∧ True) (b2 : SFBool_u) (b2_p : SFBool_wf b2 ∧ True):
-  nandb_rel b1 b2 ⌊ nandb (exist _ b1 b1_p) (exist _ b2 b2_p) ⌋.
+  nandb_rel b1 b2 ⌊ nandb (exist _ b1 b1_p) (exist _ b2 b2_p) -⌋.
 Proof.
   Opaque nandb.
   existence_lemma_pre nandb;
@@ -658,7 +658,7 @@ Theorem nandb__nandb_rel_rw
   (b2 : SFBool_u)
   (b2_p : SFBool_wf b2 ∧ True)
   (VV : SFBool_u):
-  ⌊ nandb (exist _ b1 b1_p) (exist _ b2 b2_p) ⌋ = VV ↔ nandb_rel b1 b2 VV.
+  ⌊ nandb (exist _ b1 b1_p) (exist _ b2 b2_p) -⌋ = VV ↔ nandb_rel b1 b2 VV.
 Proof.
   f__f_rel_rw.
 Qed.
@@ -670,7 +670,7 @@ Qed.
 #[global] Instance nandb_lookup_rw: dictionary rwLem nandb := { lookup' := nandb__nandb_rel_rw }.
 
 Theorem nandb__nandb_rel (b1 b2 : SFBool) (VV : SFBool_u):
-  ⌊ nandb b1 b2 ⌋ = VV ↔ nandb_rel ⌊ b1 ⌋ ⌊ b2 ⌋ VV.
+  ⌊ nandb b1 b2 -⌋ = VV ↔ nandb_rel ⌊ b1 ⌋ ⌊ b2 ⌋ VV.
 Proof.
   f__f_rel.
 Qed.
@@ -678,7 +678,7 @@ Qed.
 #[global] Hint Rewrite nandb__nandb_rel: f_rel_funct_db.
 
 Theorem nandb__nandb_rel' (b1_u b2_u : SFBool_u) (b1 b2 : SFBool) (VV : SFBool_u):
-  b1_u = ⌊ b1 ⌋ → (b2_u = ⌊ b2 ⌋ → ⌊ nandb b1 b2 ⌋ = VV ↔ nandb_rel b1_u b2_u VV).
+  b1_u = ⌊ b1 ⌋ → (b2_u = ⌊ b2 ⌋ → ⌊ nandb b1 b2 -⌋ = VV ↔ nandb_rel b1_u b2_u VV).
 Proof.
   intros -> ->. refine (nandb__nandb_rel b1 b2 VV).
 Qed.
@@ -818,7 +818,7 @@ Qed.
 #[global] Hint Rewrite negb_SFFalse_lem: f_rel_back.
 
 Theorem negb_rel_ex (lq_tmp0 : SFBool_u) (lq_tmp0_p : SFBool_wf lq_tmp0 ∧ True):
-  negb_rel lq_tmp0 ⌊ negb (exist _ lq_tmp0 lq_tmp0_p) ⌋.
+  negb_rel lq_tmp0 ⌊ negb (exist _ lq_tmp0 lq_tmp0_p) -⌋.
 Proof.
   Opaque negb.
   existence_lemma_pre negb;
@@ -835,7 +835,7 @@ Qed.
 
 Theorem negb__negb_rel_rw
   (lq_tmp0 : SFBool_u) (lq_tmp0_p : SFBool_wf lq_tmp0 ∧ True) (VV : SFBool_u):
-  ⌊ negb (exist _ lq_tmp0 lq_tmp0_p) ⌋ = VV ↔ negb_rel lq_tmp0 VV.
+  ⌊ negb (exist _ lq_tmp0 lq_tmp0_p) -⌋ = VV ↔ negb_rel lq_tmp0 VV.
 Proof.
   f__f_rel_rw.
 Qed.
@@ -847,7 +847,7 @@ Qed.
 #[global] Instance negb_lookup_rw: dictionary rwLem negb := { lookup' := negb__negb_rel_rw }.
 
 Theorem negb__negb_rel (lq_tmp0 : SFBool) (VV : SFBool_u):
-  ⌊ negb lq_tmp0 ⌋ = VV ↔ negb_rel ⌊ lq_tmp0 ⌋ VV.
+  ⌊ negb lq_tmp0 -⌋ = VV ↔ negb_rel ⌊ lq_tmp0 ⌋ VV.
 Proof.
   f__f_rel.
 Qed.
@@ -855,7 +855,7 @@ Qed.
 #[global] Hint Rewrite negb__negb_rel: f_rel_funct_db.
 
 Theorem negb__negb_rel' (lq_tmp0_u : SFBool_u) (lq_tmp0 : SFBool) (VV : SFBool_u):
-  lq_tmp0_u = ⌊ lq_tmp0 ⌋ → ⌊ negb lq_tmp0 ⌋ = VV ↔ negb_rel lq_tmp0_u VV.
+  lq_tmp0_u = ⌊ lq_tmp0 ⌋ → ⌊ negb lq_tmp0 -⌋ = VV ↔ negb_rel lq_tmp0_u VV.
 Proof.
   intros ->. refine (negb__negb_rel lq_tmp0 VV).
 Qed.
@@ -977,7 +977,7 @@ Qed.
 
 Theorem orb_rel_ex
   (b1 : SFBool_u) (b1_p : SFBool_wf b1 ∧ True) (b2 : SFBool_u) (b2_p : SFBool_wf b2 ∧ True):
-  orb_rel b1 b2 ⌊ orb (exist _ b1 b1_p) (exist _ b2 b2_p) ⌋.
+  orb_rel b1 b2 ⌊ orb (exist _ b1 b1_p) (exist _ b2 b2_p) -⌋.
 Proof.
   Opaque orb.
   existence_lemma_pre orb;
@@ -998,7 +998,7 @@ Theorem orb__orb_rel_rw
   (b2 : SFBool_u)
   (b2_p : SFBool_wf b2 ∧ True)
   (VV : SFBool_u):
-  ⌊ orb (exist _ b1 b1_p) (exist _ b2 b2_p) ⌋ = VV ↔ orb_rel b1 b2 VV.
+  ⌊ orb (exist _ b1 b1_p) (exist _ b2 b2_p) -⌋ = VV ↔ orb_rel b1 b2 VV.
 Proof.
   f__f_rel_rw.
 Qed.
@@ -1010,7 +1010,7 @@ Qed.
 #[global] Instance orb_lookup_rw: dictionary rwLem orb := { lookup' := orb__orb_rel_rw }.
 
 Theorem orb__orb_rel (b1 b2 : SFBool) (VV : SFBool_u):
-  ⌊ orb b1 b2 ⌋ = VV ↔ orb_rel ⌊ b1 ⌋ ⌊ b2 ⌋ VV.
+  ⌊ orb b1 b2 -⌋ = VV ↔ orb_rel ⌊ b1 ⌋ ⌊ b2 ⌋ VV.
 Proof.
   f__f_rel.
 Qed.
@@ -1018,7 +1018,7 @@ Qed.
 #[global] Hint Rewrite orb__orb_rel: f_rel_funct_db.
 
 Theorem orb__orb_rel' (b1_u b2_u : SFBool_u) (b1 b2 : SFBool) (VV : SFBool_u):
-  b1_u = ⌊ b1 ⌋ → (b2_u = ⌊ b2 ⌋ → ⌊ orb b1 b2 ⌋ = VV ↔ orb_rel b1_u b2_u VV).
+  b1_u = ⌊ b1 ⌋ → (b2_u = ⌊ b2 ⌋ → ⌊ orb b1 b2 -⌋ = VV ↔ orb_rel b1_u b2_u VV).
 Proof.
   intros -> ->. refine (orb__orb_rel b1 b2 VV).
 Qed.
@@ -1176,7 +1176,7 @@ Inductive SFBit_u: Type :=
 Fixpoint SFBit_wf (x : SFBit_u): Prop :=
   match x with | B0_u => True | B1_u => True end.
 
-Theorem SFBit_wf_ref [p : SFBit_u → Prop] (tm : {v: SFBit_u | SFBit_wf v ∧ p v}): SFBit_wf ⌊ tm ⌋.
+Theorem SFBit_wf_ref [p : SFBit_u → Prop] (tm : {v: SFBit_u | SFBit_wf v ∧ p v}): SFBit_wf ⌊ tm -⌋.
 Proof.
   destruct tm as [tm tm_p]. solver.
 Qed.
@@ -1242,7 +1242,7 @@ Qed.
 Fixpoint SFBin_wf (x : SFBin_u): Prop :=
   match x with | Bin0_u n => SFBin_wf n ∧ True | Bin1_u n => SFBin_wf n ∧ True | Z_u => True end.
 
-Theorem SFBin_wf_ref [p : SFBin_u → Prop] (tm : {v: SFBin_u | SFBin_wf v ∧ p v}): SFBin_wf ⌊ tm ⌋.
+Theorem SFBin_wf_ref [p : SFBin_u → Prop] (tm : {v: SFBin_u | SFBin_wf v ∧ p v}): SFBin_wf ⌊ tm -⌋.
 Proof.
   destruct tm as [tm tm_p]. solver.
 Qed.
@@ -1391,7 +1391,7 @@ Qed.
 #[global] Hint Rewrite bin_to_nat_Bin1_lem: f_rel_back.
 
 Theorem bin_to_nat_rel_ex (m : SFBin_u) (m_p : SFBin_wf m ∧ True):
-  bin_to_nat_rel m ⌊ bin_to_nat (exist _ m m_p) ⌋.
+  bin_to_nat_rel m ⌊ bin_to_nat (exist _ m m_p) -⌋.
 Proof.
   Opaque bin_to_nat.
   existence_lemma_pre bin_to_nat;
@@ -1409,7 +1409,7 @@ Qed.
 #[global] Opaque bin_to_nat.
 
 Theorem bin_to_nat__bin_to_nat_rel_rw (m : SFBin_u) (m_p : SFBin_wf m ∧ True) (VV : Z):
-  ⌊ bin_to_nat (exist _ m m_p) ⌋ = VV ↔ bin_to_nat_rel m VV.
+  ⌊ bin_to_nat (exist _ m m_p) -⌋ = VV ↔ bin_to_nat_rel m VV.
 Proof.
   f__f_rel_rw.
 Qed.
@@ -1422,7 +1422,7 @@ Qed.
     lookup' := bin_to_nat__bin_to_nat_rel_rw }.
 
 Theorem bin_to_nat__bin_to_nat_rel (m : SFBin) (VV : Z):
-  ⌊ bin_to_nat m ⌋ = VV ↔ bin_to_nat_rel ⌊ m ⌋ VV.
+  ⌊ bin_to_nat m -⌋ = VV ↔ bin_to_nat_rel ⌊ m ⌋ VV.
 Proof.
   f__f_rel.
 Qed.
@@ -1430,7 +1430,7 @@ Qed.
 #[global] Hint Rewrite bin_to_nat__bin_to_nat_rel: f_rel_funct_db.
 
 Theorem bin_to_nat__bin_to_nat_rel' (m_u : SFBin_u) (m : SFBin) (VV : Z):
-  m_u = ⌊ m ⌋ → ⌊ bin_to_nat m ⌋ = VV ↔ bin_to_nat_rel m_u VV.
+  m_u = ⌊ m ⌋ → ⌊ bin_to_nat m -⌋ = VV ↔ bin_to_nat_rel m_u VV.
 Proof.
   intros ->. refine (bin_to_nat__bin_to_nat_rel m VV).
 Qed.
@@ -1536,12 +1536,14 @@ Qed.
 
 #[global] Hint Rewrite incr_Bin1_lem: f_rel_back.
 
-Theorem incr_rel_ex (m : SFBin_u) (m_p : SFBin_wf m ∧ True): incr_rel m ⌊ incr (exist _ m m_p) ⌋.
+Theorem incr_rel_ex (m : SFBin_u) (m_p : SFBin_wf m ∧ True): incr_rel m ⌊ incr (exist _ m m_p) -⌋.
 Proof.
   Opaque incr.
   existence_lemma_pre incr;
   induction m as [m' _| m' IH_m'|];
-  [fix_notations | fix_notations | fix_notations];
+  [fix_notations |
+   fix_notations; pose proof (IH_m' ltac:(try clear IH_m'; solver)) as IH_34714780; try clear IH_m' |
+   fix_notations];
   simpl in *.
   Transparent incr.
   all: existence_lemma_quicksolve incr; f__f_rel_ex_body; f_rel_finish.
@@ -1552,7 +1554,7 @@ Qed.
 #[global] Opaque incr.
 
 Theorem incr__incr_rel_rw (m : SFBin_u) (m_p : SFBin_wf m ∧ True) (VV : SFBin_u):
-  ⌊ incr (exist _ m m_p) ⌋ = VV ↔ incr_rel m VV.
+  ⌊ incr (exist _ m m_p) -⌋ = VV ↔ incr_rel m VV.
 Proof.
   f__f_rel_rw.
 Qed.
@@ -1563,7 +1565,7 @@ Qed.
 
 #[global] Instance incr_lookup_rw: dictionary rwLem incr := { lookup' := incr__incr_rel_rw }.
 
-Theorem incr__incr_rel (m : SFBin) (VV : SFBin_u): ⌊ incr m ⌋ = VV ↔ incr_rel ⌊ m ⌋ VV.
+Theorem incr__incr_rel (m : SFBin) (VV : SFBin_u): ⌊ incr m -⌋ = VV ↔ incr_rel ⌊ m ⌋ VV.
 Proof.
   f__f_rel.
 Qed.
@@ -1571,7 +1573,7 @@ Qed.
 #[global] Hint Rewrite incr__incr_rel: f_rel_funct_db.
 
 Theorem incr__incr_rel' (m_u : SFBin_u) (m : SFBin) (VV : SFBin_u):
-  m_u = ⌊ m ⌋ → ⌊ incr m ⌋ = VV ↔ incr_rel m_u VV.
+  m_u = ⌊ m ⌋ → ⌊ incr m -⌋ = VV ↔ incr_rel m_u VV.
 Proof.
   intros ->. refine (incr__incr_rel m VV).
 Qed.
@@ -1713,7 +1715,7 @@ Inductive RGB_u: Type :=
 Fixpoint RGB_wf (x : RGB_u): Prop :=
   match x with | Blue_u => True | Green_u => True | Red_u => True end.
 
-Theorem RGB_wf_ref [p : RGB_u → Prop] (tm : {v: RGB_u | RGB_wf v ∧ p v}): RGB_wf ⌊ tm ⌋.
+Theorem RGB_wf_ref [p : RGB_u → Prop] (tm : {v: RGB_u | RGB_wf v ∧ p v}): RGB_wf ⌊ tm -⌋.
 Proof.
   destruct tm as [tm tm_p]. solver.
 Qed.
@@ -1789,7 +1791,7 @@ Fixpoint OtherNat_wf (x : OtherNat_u): Prop :=
   match x with | Stop_u => True | Tick_u VV => OtherNat_wf VV ∧ True end.
 
 Theorem OtherNat_wf_ref [p : OtherNat_u → Prop] (tm : {v: OtherNat_u | OtherNat_wf v ∧ p v}):
-  OtherNat_wf ⌊ tm ⌋.
+  OtherNat_wf ⌊ tm -⌋.
 Proof.
   destruct tm as [tm tm_p]. solver.
 Qed.
@@ -1867,7 +1869,7 @@ Fixpoint Nibble_wf (x : Nibble_u): Prop :=
   end.
 
 Theorem Nibble_wf_ref [p : Nibble_u → Prop] (tm : {v: Nibble_u | Nibble_wf v ∧ p v}):
-  Nibble_wf ⌊ tm ⌋.
+  Nibble_wf ⌊ tm -⌋.
 Proof.
   destruct tm as [tm tm_p]. solver.
 Qed.
@@ -1975,7 +1977,7 @@ Qed.
 Fixpoint MyNat_wf (x : MyNat_u): Prop :=
   match x with | O_u => True | S_u VV => MyNat_wf VV ∧ True end.
 
-Theorem MyNat_wf_ref [p : MyNat_u → Prop] (tm : {v: MyNat_u | MyNat_wf v ∧ p v}): MyNat_wf ⌊ tm ⌋.
+Theorem MyNat_wf_ref [p : MyNat_u → Prop] (tm : {v: MyNat_u | MyNat_wf v ∧ p v}): MyNat_wf ⌊ tm -⌋.
 Proof.
   destruct tm as [tm tm_p]. solver.
 Qed.
@@ -2088,7 +2090,7 @@ Qed.
 #[global] Hint Rewrite eqb_S_S_lem: f_rel_back.
 
 Theorem eqb_rel_ex (n : MyNat_u) (n_p : MyNat_wf n ∧ True) (m : MyNat_u) (m_p : MyNat_wf m ∧ True):
-  eqb_rel n m ⌊ eqb (exist _ n n_p) (exist _ m m_p) ⌋.
+  eqb_rel n m ⌊ eqb (exist _ n n_p) (exist _ m m_p) -⌋.
 Proof.
   Opaque eqb.
   existence_lemma_pre eqb;
@@ -2111,7 +2113,7 @@ Qed.
 
 Theorem eqb__eqb_rel_rw
   (n : MyNat_u) (n_p : MyNat_wf n ∧ True) (m : MyNat_u) (m_p : MyNat_wf m ∧ True) (VV : SFBool_u):
-  ⌊ eqb (exist _ n n_p) (exist _ m m_p) ⌋ = VV ↔ eqb_rel n m VV.
+  ⌊ eqb (exist _ n n_p) (exist _ m m_p) -⌋ = VV ↔ eqb_rel n m VV.
 Proof.
   f__f_rel_rw.
 Qed.
@@ -2122,7 +2124,7 @@ Qed.
 
 #[global] Instance eqb_lookup_rw: dictionary rwLem eqb := { lookup' := eqb__eqb_rel_rw }.
 
-Theorem eqb__eqb_rel (n m : MyNat) (VV : SFBool_u): ⌊ eqb n m ⌋ = VV ↔ eqb_rel ⌊ n ⌋ ⌊ m ⌋ VV.
+Theorem eqb__eqb_rel (n m : MyNat) (VV : SFBool_u): ⌊ eqb n m -⌋ = VV ↔ eqb_rel ⌊ n ⌋ ⌊ m ⌋ VV.
 Proof.
   f__f_rel.
 Qed.
@@ -2130,7 +2132,7 @@ Qed.
 #[global] Hint Rewrite eqb__eqb_rel: f_rel_funct_db.
 
 Theorem eqb__eqb_rel' (n_u m_u : MyNat_u) (n m : MyNat) (VV : SFBool_u):
-  n_u = ⌊ n ⌋ → (m_u = ⌊ m ⌋ → ⌊ eqb n m ⌋ = VV ↔ eqb_rel n_u m_u VV).
+  n_u = ⌊ n ⌋ → (m_u = ⌊ m ⌋ → ⌊ eqb n m -⌋ = VV ↔ eqb_rel n_u m_u VV).
 Proof.
   intros -> ->. refine (eqb__eqb_rel n m VV).
 Qed.
@@ -2228,7 +2230,7 @@ Qed.
 #[global] Hint Rewrite leb_S_S_lem: f_rel_back.
 
 Theorem leb_rel_ex (n : MyNat_u) (n_p : MyNat_wf n ∧ True) (m : MyNat_u) (m_p : MyNat_wf m ∧ True):
-  leb_rel n m ⌊ leb (exist _ n n_p) (exist _ m m_p) ⌋.
+  leb_rel n m ⌊ leb (exist _ n n_p) (exist _ m m_p) -⌋.
 Proof.
   Opaque leb.
   existence_lemma_pre leb;
@@ -2250,7 +2252,7 @@ Qed.
 
 Theorem leb__leb_rel_rw
   (n : MyNat_u) (n_p : MyNat_wf n ∧ True) (m : MyNat_u) (m_p : MyNat_wf m ∧ True) (VV : SFBool_u):
-  ⌊ leb (exist _ n n_p) (exist _ m m_p) ⌋ = VV ↔ leb_rel n m VV.
+  ⌊ leb (exist _ n n_p) (exist _ m m_p) -⌋ = VV ↔ leb_rel n m VV.
 Proof.
   f__f_rel_rw.
 Qed.
@@ -2261,7 +2263,7 @@ Qed.
 
 #[global] Instance leb_lookup_rw: dictionary rwLem leb := { lookup' := leb__leb_rel_rw }.
 
-Theorem leb__leb_rel (n m : MyNat) (VV : SFBool_u): ⌊ leb n m ⌋ = VV ↔ leb_rel ⌊ n ⌋ ⌊ m ⌋ VV.
+Theorem leb__leb_rel (n m : MyNat) (VV : SFBool_u): ⌊ leb n m -⌋ = VV ↔ leb_rel ⌊ n ⌋ ⌊ m ⌋ VV.
 Proof.
   f__f_rel.
 Qed.
@@ -2269,7 +2271,7 @@ Qed.
 #[global] Hint Rewrite leb__leb_rel: f_rel_funct_db.
 
 Theorem leb__leb_rel' (n_u m_u : MyNat_u) (n m : MyNat) (VV : SFBool_u):
-  n_u = ⌊ n ⌋ → (m_u = ⌊ m ⌋ → ⌊ leb n m ⌋ = VV ↔ leb_rel n_u m_u VV).
+  n_u = ⌊ n ⌋ → (m_u = ⌊ m ⌋ → ⌊ leb n m -⌋ = VV ↔ leb_rel n_u m_u VV).
 Proof.
   intros -> ->. refine (leb__leb_rel n m VV).
 Qed.
@@ -2378,7 +2380,7 @@ Qed.
 #[global] Hint Rewrite ltb_S_S_lem: f_rel_back.
 
 Theorem ltb_rel_ex (n : MyNat_u) (n_p : MyNat_wf n ∧ True) (m : MyNat_u) (m_p : MyNat_wf m ∧ True):
-  ltb_rel n m ⌊ ltb (exist _ n n_p) (exist _ m m_p) ⌋.
+  ltb_rel n m ⌊ ltb (exist _ n n_p) (exist _ m m_p) -⌋.
 Proof.
   Opaque ltb.
   existence_lemma_pre ltb;
@@ -2401,7 +2403,7 @@ Qed.
 
 Theorem ltb__ltb_rel_rw
   (n : MyNat_u) (n_p : MyNat_wf n ∧ True) (m : MyNat_u) (m_p : MyNat_wf m ∧ True) (VV : SFBool_u):
-  ⌊ ltb (exist _ n n_p) (exist _ m m_p) ⌋ = VV ↔ ltb_rel n m VV.
+  ⌊ ltb (exist _ n n_p) (exist _ m m_p) -⌋ = VV ↔ ltb_rel n m VV.
 Proof.
   f__f_rel_rw.
 Qed.
@@ -2412,7 +2414,7 @@ Qed.
 
 #[global] Instance ltb_lookup_rw: dictionary rwLem ltb := { lookup' := ltb__ltb_rel_rw }.
 
-Theorem ltb__ltb_rel (n m : MyNat) (VV : SFBool_u): ⌊ ltb n m ⌋ = VV ↔ ltb_rel ⌊ n ⌋ ⌊ m ⌋ VV.
+Theorem ltb__ltb_rel (n m : MyNat) (VV : SFBool_u): ⌊ ltb n m -⌋ = VV ↔ ltb_rel ⌊ n ⌋ ⌊ m ⌋ VV.
 Proof.
   f__f_rel.
 Qed.
@@ -2420,7 +2422,7 @@ Qed.
 #[global] Hint Rewrite ltb__ltb_rel: f_rel_funct_db.
 
 Theorem ltb__ltb_rel' (n_u m_u : MyNat_u) (n m : MyNat) (VV : SFBool_u):
-  n_u = ⌊ n ⌋ → (m_u = ⌊ m ⌋ → ⌊ ltb n m ⌋ = VV ↔ ltb_rel n_u m_u VV).
+  n_u = ⌊ n ⌋ → (m_u = ⌊ m ⌋ → ⌊ ltb n m -⌋ = VV ↔ ltb_rel n_u m_u VV).
 Proof.
   intros -> ->. refine (ltb__ltb_rel n m VV).
 Qed.
@@ -2521,7 +2523,7 @@ Qed.
 
 Theorem minus_rel_ex
   (n : MyNat_u) (n_p : MyNat_wf n ∧ True) (m : MyNat_u) (m_p : MyNat_wf m ∧ True):
-  minus_rel n m ⌊ minus (exist _ n n_p) (exist _ m m_p) ⌋.
+  minus_rel n m ⌊ minus (exist _ n n_p) (exist _ m m_p) -⌋.
 Proof.
   Opaque minus.
   existence_lemma_pre minus;
@@ -2546,7 +2548,7 @@ Qed.
 
 Theorem minus__minus_rel_rw
   (n : MyNat_u) (n_p : MyNat_wf n ∧ True) (m : MyNat_u) (m_p : MyNat_wf m ∧ True) (VV : MyNat_u):
-  ⌊ minus (exist _ n n_p) (exist _ m m_p) ⌋ = VV ↔ minus_rel n m VV.
+  ⌊ minus (exist _ n n_p) (exist _ m m_p) -⌋ = VV ↔ minus_rel n m VV.
 Proof.
   f__f_rel_rw.
 Qed.
@@ -2558,7 +2560,7 @@ Qed.
 #[global] Instance minus_lookup_rw: dictionary rwLem minus := { lookup' := minus__minus_rel_rw }.
 
 Theorem minus__minus_rel (n m : MyNat) (VV : MyNat_u):
-  ⌊ minus n m ⌋ = VV ↔ minus_rel ⌊ n ⌋ ⌊ m ⌋ VV.
+  ⌊ minus n m -⌋ = VV ↔ minus_rel ⌊ n ⌋ ⌊ m ⌋ VV.
 Proof.
   f__f_rel.
 Qed.
@@ -2566,7 +2568,7 @@ Qed.
 #[global] Hint Rewrite minus__minus_rel: f_rel_funct_db.
 
 Theorem minus__minus_rel' (n_u m_u : MyNat_u) (n m : MyNat) (VV : MyNat_u):
-  n_u = ⌊ n ⌋ → (m_u = ⌊ m ⌋ → ⌊ minus n m ⌋ = VV ↔ minus_rel n_u m_u VV).
+  n_u = ⌊ n ⌋ → (m_u = ⌊ m ⌋ → ⌊ minus n m -⌋ = VV ↔ minus_rel n_u m_u VV).
 Proof.
   intros -> ->. refine (minus__minus_rel n m VV).
 Qed.
@@ -2651,7 +2653,7 @@ Qed.
 
 #[global] Hint Rewrite one_inv_lem: f_rel_back.
 
-Theorem one_rel_ex : one_rel ⌊ one ⌋.
+Theorem one_rel_ex : one_rel ⌊ one -⌋.
 Proof.
   Opaque one.
   existence_lemma_pre one; fix_notations; simpl in *.
@@ -2663,7 +2665,7 @@ Qed.
 
 #[global] Opaque one.
 
-Theorem one__one_rel_rw (VV : MyNat_u): ⌊ one ⌋ = VV ↔ one_rel VV.
+Theorem one__one_rel_rw (VV : MyNat_u): ⌊ one -⌋ = VV ↔ one_rel VV.
 Proof.
   f__f_rel_rw.
 Qed.
@@ -2674,14 +2676,14 @@ Qed.
 
 #[global] Instance one_lookup_rw: dictionary rwLem one := { lookup' := one__one_rel_rw }.
 
-Theorem one__one_rel (VV : MyNat_u): ⌊ one ⌋ = VV ↔ one_rel VV.
+Theorem one__one_rel (VV : MyNat_u): ⌊ one -⌋ = VV ↔ one_rel VV.
 Proof.
   f__f_rel.
 Qed.
 
 #[global] Hint Rewrite one__one_rel: f_rel_funct_db.
 
-Theorem one__one_rel' (VV : MyNat_u): ⌊ one ⌋ = VV ↔ one_rel VV.
+Theorem one__one_rel' (VV : MyNat_u): ⌊ one -⌋ = VV ↔ one_rel VV.
 Proof.
   intros. refine (one__one_rel VV).
 Qed.
@@ -2744,12 +2746,15 @@ Qed.
 #[global] Hint Rewrite plus_S_x_lem: f_rel_back.
 
 Theorem plus_rel_ex (n : MyNat_u) (n_p : MyNat_wf n ∧ True) (m : MyNat_u) (m_p : MyNat_wf m ∧ True):
-  plus_rel n m ⌊ plus (exist _ n n_p) (exist _ m m_p) ⌋.
+  plus_rel n m ⌊ plus (exist _ n n_p) (exist _ m m_p) -⌋.
 Proof.
   Opaque plus.
   existence_lemma_pre plus;
   try revert m_p; generalize dependent m; induction n as [| n' IH_n']; intros;
-  [fix_notations | fix_notations];
+  [fix_notations |
+   fix_notations;
+   pose proof (IH_n' ltac:(try clear IH_n'; solver) m ltac:(try clear IH_n'; solver)) as IH_47989236;
+   try clear IH_n'];
   simpl in *.
   Transparent plus.
   all: existence_lemma_quicksolve plus; f__f_rel_ex_body; f_rel_finish.
@@ -2761,7 +2766,7 @@ Qed.
 
 Theorem plus__plus_rel_rw
   (n : MyNat_u) (n_p : MyNat_wf n ∧ True) (m : MyNat_u) (m_p : MyNat_wf m ∧ True) (VV : MyNat_u):
-  ⌊ plus (exist _ n n_p) (exist _ m m_p) ⌋ = VV ↔ plus_rel n m VV.
+  ⌊ plus (exist _ n n_p) (exist _ m m_p) -⌋ = VV ↔ plus_rel n m VV.
 Proof.
   f__f_rel_rw.
 Qed.
@@ -2772,7 +2777,7 @@ Qed.
 
 #[global] Instance plus_lookup_rw: dictionary rwLem plus := { lookup' := plus__plus_rel_rw }.
 
-Theorem plus__plus_rel (n m : MyNat) (VV : MyNat_u): ⌊ plus n m ⌋ = VV ↔ plus_rel ⌊ n ⌋ ⌊ m ⌋ VV.
+Theorem plus__plus_rel (n m : MyNat) (VV : MyNat_u): ⌊ plus n m -⌋ = VV ↔ plus_rel ⌊ n ⌋ ⌊ m ⌋ VV.
 Proof.
   f__f_rel.
 Qed.
@@ -2780,7 +2785,7 @@ Qed.
 #[global] Hint Rewrite plus__plus_rel: f_rel_funct_db.
 
 Theorem plus__plus_rel' (n_u m_u : MyNat_u) (n m : MyNat) (VV : MyNat_u):
-  n_u = ⌊ n ⌋ → (m_u = ⌊ m ⌋ → ⌊ plus n m ⌋ = VV ↔ plus_rel n_u m_u VV).
+  n_u = ⌊ n ⌋ → (m_u = ⌊ m ⌋ → ⌊ plus n m -⌋ = VV ↔ plus_rel n_u m_u VV).
 Proof.
   intros -> ->. refine (plus__plus_rel n m VV).
 Qed.
@@ -2949,12 +2954,15 @@ Qed.
 #[global] Hint Rewrite mult_S_x_lem: f_rel_back.
 
 Theorem mult_rel_ex (n : MyNat_u) (n_p : MyNat_wf n ∧ True) (m : MyNat_u) (m_p : MyNat_wf m ∧ True):
-  mult_rel n m ⌊ mult (exist _ n n_p) (exist _ m m_p) ⌋.
+  mult_rel n m ⌊ mult (exist _ n n_p) (exist _ m m_p) -⌋.
 Proof.
   Opaque mult.
   existence_lemma_pre mult;
   try revert m_p; generalize dependent m; induction n as [| n' IH_n']; intros;
-  [fix_notations | fix_notations];
+  [fix_notations |
+   fix_notations;
+   pose proof (IH_n' ltac:(try clear IH_n'; solver) m ltac:(try clear IH_n'; solver)) as IH_47989236;
+   try clear IH_n'];
   simpl in *.
   Transparent mult.
   all: existence_lemma_quicksolve mult; f__f_rel_ex_body; f_rel_finish.
@@ -2966,7 +2974,7 @@ Qed.
 
 Theorem mult__mult_rel_rw
   (n : MyNat_u) (n_p : MyNat_wf n ∧ True) (m : MyNat_u) (m_p : MyNat_wf m ∧ True) (VV : MyNat_u):
-  ⌊ mult (exist _ n n_p) (exist _ m m_p) ⌋ = VV ↔ mult_rel n m VV.
+  ⌊ mult (exist _ n n_p) (exist _ m m_p) -⌋ = VV ↔ mult_rel n m VV.
 Proof.
   f__f_rel_rw.
 Qed.
@@ -2977,7 +2985,7 @@ Qed.
 
 #[global] Instance mult_lookup_rw: dictionary rwLem mult := { lookup' := mult__mult_rel_rw }.
 
-Theorem mult__mult_rel (n m : MyNat) (VV : MyNat_u): ⌊ mult n m ⌋ = VV ↔ mult_rel ⌊ n ⌋ ⌊ m ⌋ VV.
+Theorem mult__mult_rel (n m : MyNat) (VV : MyNat_u): ⌊ mult n m -⌋ = VV ↔ mult_rel ⌊ n ⌋ ⌊ m ⌋ VV.
 Proof.
   f__f_rel.
 Qed.
@@ -2985,7 +2993,7 @@ Qed.
 #[global] Hint Rewrite mult__mult_rel: f_rel_funct_db.
 
 Theorem mult__mult_rel' (n_u m_u : MyNat_u) (n m : MyNat) (VV : MyNat_u):
-  n_u = ⌊ n ⌋ → (m_u = ⌊ m ⌋ → ⌊ mult n m ⌋ = VV ↔ mult_rel n_u m_u VV).
+  n_u = ⌊ n ⌋ → (m_u = ⌊ m ⌋ → ⌊ mult n m -⌋ = VV ↔ mult_rel n_u m_u VV).
 Proof.
   intros -> ->. refine (mult__mult_rel n m VV).
 Qed.
@@ -3076,12 +3084,13 @@ Qed.
 #[global] Hint Rewrite factorial_S_lem: f_rel_back.
 
 Theorem factorial_rel_ex (lq_tmp0 : MyNat_u) (lq_tmp0_p : MyNat_wf lq_tmp0 ∧ True):
-  factorial_rel lq_tmp0 ⌊ factorial (exist _ lq_tmp0 lq_tmp0_p) ⌋.
+  factorial_rel lq_tmp0 ⌊ factorial (exist _ lq_tmp0 lq_tmp0_p) -⌋.
 Proof.
   Opaque factorial.
   existence_lemma_pre factorial;
   induction lq_tmp0 as [| n' IH_n'];
-  [fix_notations | fix_notations];
+  [fix_notations |
+   fix_notations; pose proof (IH_n' ltac:(try clear IH_n'; solver)) as IH_36186333; try clear IH_n'];
   simpl in *.
   Transparent factorial.
   all: existence_lemma_quicksolve factorial; f__f_rel_ex_body; f_rel_finish.
@@ -3093,7 +3102,7 @@ Qed.
 
 Theorem factorial__factorial_rel_rw
   (lq_tmp0 : MyNat_u) (lq_tmp0_p : MyNat_wf lq_tmp0 ∧ True) (VV : MyNat_u):
-  ⌊ factorial (exist _ lq_tmp0 lq_tmp0_p) ⌋ = VV ↔ factorial_rel lq_tmp0 VV.
+  ⌊ factorial (exist _ lq_tmp0 lq_tmp0_p) -⌋ = VV ↔ factorial_rel lq_tmp0 VV.
 Proof.
   f__f_rel_rw.
 Qed.
@@ -3106,7 +3115,7 @@ Qed.
     lookup' := factorial__factorial_rel_rw }.
 
 Theorem factorial__factorial_rel (lq_tmp0 : MyNat) (VV : MyNat_u):
-  ⌊ factorial lq_tmp0 ⌋ = VV ↔ factorial_rel ⌊ lq_tmp0 ⌋ VV.
+  ⌊ factorial lq_tmp0 -⌋ = VV ↔ factorial_rel ⌊ lq_tmp0 ⌋ VV.
 Proof.
   f__f_rel.
 Qed.
@@ -3114,7 +3123,7 @@ Qed.
 #[global] Hint Rewrite factorial__factorial_rel: f_rel_funct_db.
 
 Theorem factorial__factorial_rel' (lq_tmp0_u : MyNat_u) (lq_tmp0 : MyNat) (VV : MyNat_u):
-  lq_tmp0_u = ⌊ lq_tmp0 ⌋ → ⌊ factorial lq_tmp0 ⌋ = VV ↔ factorial_rel lq_tmp0_u VV.
+  lq_tmp0_u = ⌊ lq_tmp0 ⌋ → ⌊ factorial lq_tmp0 -⌋ = VV ↔ factorial_rel lq_tmp0_u VV.
 Proof.
   intros ->. refine (factorial__factorial_rel lq_tmp0 VV).
 Qed.
@@ -3448,7 +3457,7 @@ Qed.
 #[global] Hint Rewrite pred_S_lem: f_rel_back.
 
 Theorem pred_rel_ex (lq_tmp0 : MyNat_u) (lq_tmp0_p : MyNat_wf lq_tmp0 ∧ True):
-  pred_rel lq_tmp0 ⌊ pred (exist _ lq_tmp0 lq_tmp0_p) ⌋.
+  pred_rel lq_tmp0 ⌊ pred (exist _ lq_tmp0 lq_tmp0_p) -⌋.
 Proof.
   Opaque pred.
   existence_lemma_pre pred;
@@ -3464,7 +3473,7 @@ Qed.
 #[global] Opaque pred.
 
 Theorem pred__pred_rel_rw (lq_tmp0 : MyNat_u) (lq_tmp0_p : MyNat_wf lq_tmp0 ∧ True) (VV : MyNat_u):
-  ⌊ pred (exist _ lq_tmp0 lq_tmp0_p) ⌋ = VV ↔ pred_rel lq_tmp0 VV.
+  ⌊ pred (exist _ lq_tmp0 lq_tmp0_p) -⌋ = VV ↔ pred_rel lq_tmp0 VV.
 Proof.
   f__f_rel_rw.
 Qed.
@@ -3476,7 +3485,7 @@ Qed.
 #[global] Instance pred_lookup_rw: dictionary rwLem pred := { lookup' := pred__pred_rel_rw }.
 
 Theorem pred__pred_rel (lq_tmp0 : MyNat) (VV : MyNat_u):
-  ⌊ pred lq_tmp0 ⌋ = VV ↔ pred_rel ⌊ lq_tmp0 ⌋ VV.
+  ⌊ pred lq_tmp0 -⌋ = VV ↔ pred_rel ⌊ lq_tmp0 ⌋ VV.
 Proof.
   f__f_rel.
 Qed.
@@ -3484,7 +3493,7 @@ Qed.
 #[global] Hint Rewrite pred__pred_rel: f_rel_funct_db.
 
 Theorem pred__pred_rel' (lq_tmp0_u : MyNat_u) (lq_tmp0 : MyNat) (VV : MyNat_u):
-  lq_tmp0_u = ⌊ lq_tmp0 ⌋ → ⌊ pred lq_tmp0 ⌋ = VV ↔ pred_rel lq_tmp0_u VV.
+  lq_tmp0_u = ⌊ lq_tmp0 ⌋ → ⌊ pred lq_tmp0 -⌋ = VV ↔ pred_rel lq_tmp0_u VV.
 Proof.
   intros ->. refine (pred__pred_rel lq_tmp0 VV).
 Qed.
@@ -3580,12 +3589,15 @@ Theorem sf_exp_rel_ex
   (base_p : MyNat_wf base ∧ True)
   (power : MyNat_u)
   (power_p : MyNat_wf power ∧ True):
-  sf_exp_rel base power ⌊ sf_exp (exist _ base base_p) (exist _ power power_p) ⌋.
+  sf_exp_rel base power ⌊ sf_exp (exist _ base base_p) (exist _ power power_p) -⌋.
 Proof.
   Opaque sf_exp.
   existence_lemma_pre sf_exp;
   try revert base_p; generalize dependent base; induction power as [| p IH_p]; intros;
-  [fix_notations | fix_notations];
+  [fix_notations |
+   fix_notations;
+   pose proof (IH_p ltac:(try clear IH_p; solver) base ltac:(try clear IH_p; solver)) as IH_73738881;
+   try clear IH_p];
   simpl in *.
   Transparent sf_exp.
   all: existence_lemma_quicksolve sf_exp; f__f_rel_ex_body; f_rel_finish.
@@ -3601,7 +3613,7 @@ Theorem sf_exp__sf_exp_rel_rw
   (power : MyNat_u)
   (power_p : MyNat_wf power ∧ True)
   (VV : MyNat_u):
-  ⌊ sf_exp (exist _ base base_p) (exist _ power power_p) ⌋ = VV ↔ sf_exp_rel base power VV.
+  ⌊ sf_exp (exist _ base base_p) (exist _ power power_p) -⌋ = VV ↔ sf_exp_rel base power VV.
 Proof.
   f__f_rel_rw.
 Qed.
@@ -3614,7 +3626,7 @@ Qed.
     lookup' := sf_exp__sf_exp_rel_rw }.
 
 Theorem sf_exp__sf_exp_rel (base power : MyNat) (VV : MyNat_u):
-  ⌊ sf_exp base power ⌋ = VV ↔ sf_exp_rel ⌊ base ⌋ ⌊ power ⌋ VV.
+  ⌊ sf_exp base power -⌋ = VV ↔ sf_exp_rel ⌊ base ⌋ ⌊ power ⌋ VV.
 Proof.
   f__f_rel.
 Qed.
@@ -3623,7 +3635,7 @@ Qed.
 
 Theorem sf_exp__sf_exp_rel' (base_u power_u : MyNat_u) (base power : MyNat) (VV : MyNat_u):
   base_u = ⌊ base ⌋
-  → (power_u = ⌊ power ⌋ → ⌊ sf_exp base power ⌋ = VV ↔ sf_exp_rel base_u power_u VV).
+  → (power_u = ⌊ power ⌋ → ⌊ sf_exp base power -⌋ = VV ↔ sf_exp_rel base_u power_u VV).
 Proof.
   intros -> ->. refine (sf_exp__sf_exp_rel base power VV).
 Qed.
@@ -3702,7 +3714,7 @@ Qed.
 
 #[global] Hint Rewrite two_inv_lem: f_rel_back.
 
-Theorem two_rel_ex : two_rel ⌊ two ⌋.
+Theorem two_rel_ex : two_rel ⌊ two -⌋.
 Proof.
   Opaque two.
   existence_lemma_pre two; fix_notations; simpl in *.
@@ -3714,7 +3726,7 @@ Qed.
 
 #[global] Opaque two.
 
-Theorem two__two_rel_rw (VV : MyNat_u): ⌊ two ⌋ = VV ↔ two_rel VV.
+Theorem two__two_rel_rw (VV : MyNat_u): ⌊ two -⌋ = VV ↔ two_rel VV.
 Proof.
   f__f_rel_rw.
 Qed.
@@ -3725,14 +3737,14 @@ Qed.
 
 #[global] Instance two_lookup_rw: dictionary rwLem two := { lookup' := two__two_rel_rw }.
 
-Theorem two__two_rel (VV : MyNat_u): ⌊ two ⌋ = VV ↔ two_rel VV.
+Theorem two__two_rel (VV : MyNat_u): ⌊ two -⌋ = VV ↔ two_rel VV.
 Proof.
   f__f_rel.
 Qed.
 
 #[global] Hint Rewrite two__two_rel: f_rel_funct_db.
 
-Theorem two__two_rel' (VV : MyNat_u): ⌊ two ⌋ = VV ↔ two_rel VV.
+Theorem two__two_rel' (VV : MyNat_u): ⌊ two -⌋ = VV ↔ two_rel VV.
 Proof.
   intros. refine (two__two_rel VV).
 Qed.
@@ -3810,7 +3822,7 @@ Qed.
 
 #[global] Hint Rewrite three_inv_lem: f_rel_back.
 
-Theorem three_rel_ex : three_rel ⌊ three ⌋.
+Theorem three_rel_ex : three_rel ⌊ three -⌋.
 Proof.
   Opaque three.
   existence_lemma_pre three; fix_notations; simpl in *.
@@ -3822,7 +3834,7 @@ Qed.
 
 #[global] Opaque three.
 
-Theorem three__three_rel_rw (VV : MyNat_u): ⌊ three ⌋ = VV ↔ three_rel VV.
+Theorem three__three_rel_rw (VV : MyNat_u): ⌊ three -⌋ = VV ↔ three_rel VV.
 Proof.
   f__f_rel_rw.
 Qed.
@@ -3833,14 +3845,14 @@ Qed.
 
 #[global] Instance three_lookup_rw: dictionary rwLem three := { lookup' := three__three_rel_rw }.
 
-Theorem three__three_rel (VV : MyNat_u): ⌊ three ⌋ = VV ↔ three_rel VV.
+Theorem three__three_rel (VV : MyNat_u): ⌊ three -⌋ = VV ↔ three_rel VV.
 Proof.
   f__f_rel.
 Qed.
 
 #[global] Hint Rewrite three__three_rel: f_rel_funct_db.
 
-Theorem three__three_rel' (VV : MyNat_u): ⌊ three ⌋ = VV ↔ three_rel VV.
+Theorem three__three_rel' (VV : MyNat_u): ⌊ three -⌋ = VV ↔ three_rel VV.
 Proof.
   intros. refine (three__three_rel VV).
 Qed.
@@ -3891,7 +3903,7 @@ Qed.
 
 #[global] Hint Rewrite four_inv_lem: f_rel_back.
 
-Theorem four_rel_ex : four_rel ⌊ four ⌋.
+Theorem four_rel_ex : four_rel ⌊ four -⌋.
 Proof.
   Opaque four.
   existence_lemma_pre four; fix_notations; simpl in *.
@@ -3903,7 +3915,7 @@ Qed.
 
 #[global] Opaque four.
 
-Theorem four__four_rel_rw (VV : MyNat_u): ⌊ four ⌋ = VV ↔ four_rel VV.
+Theorem four__four_rel_rw (VV : MyNat_u): ⌊ four -⌋ = VV ↔ four_rel VV.
 Proof.
   f__f_rel_rw.
 Qed.
@@ -3914,14 +3926,14 @@ Qed.
 
 #[global] Instance four_lookup_rw: dictionary rwLem four := { lookup' := four__four_rel_rw }.
 
-Theorem four__four_rel (VV : MyNat_u): ⌊ four ⌋ = VV ↔ four_rel VV.
+Theorem four__four_rel (VV : MyNat_u): ⌊ four -⌋ = VV ↔ four_rel VV.
 Proof.
   f__f_rel.
 Qed.
 
 #[global] Hint Rewrite four__four_rel: f_rel_funct_db.
 
-Theorem four__four_rel' (VV : MyNat_u): ⌊ four ⌋ = VV ↔ four_rel VV.
+Theorem four__four_rel' (VV : MyNat_u): ⌊ four -⌋ = VV ↔ four_rel VV.
 Proof.
   intros. refine (four__four_rel VV).
 Qed.
@@ -3972,7 +3984,7 @@ Qed.
 
 #[global] Hint Rewrite five_inv_lem: f_rel_back.
 
-Theorem five_rel_ex : five_rel ⌊ five ⌋.
+Theorem five_rel_ex : five_rel ⌊ five -⌋.
 Proof.
   Opaque five.
   existence_lemma_pre five; fix_notations; simpl in *.
@@ -3984,7 +3996,7 @@ Qed.
 
 #[global] Opaque five.
 
-Theorem five__five_rel_rw (VV : MyNat_u): ⌊ five ⌋ = VV ↔ five_rel VV.
+Theorem five__five_rel_rw (VV : MyNat_u): ⌊ five -⌋ = VV ↔ five_rel VV.
 Proof.
   f__f_rel_rw.
 Qed.
@@ -3995,14 +4007,14 @@ Qed.
 
 #[global] Instance five_lookup_rw: dictionary rwLem five := { lookup' := five__five_rel_rw }.
 
-Theorem five__five_rel (VV : MyNat_u): ⌊ five ⌋ = VV ↔ five_rel VV.
+Theorem five__five_rel (VV : MyNat_u): ⌊ five -⌋ = VV ↔ five_rel VV.
 Proof.
   f__f_rel.
 Qed.
 
 #[global] Hint Rewrite five__five_rel: f_rel_funct_db.
 
-Theorem five__five_rel' (VV : MyNat_u): ⌊ five ⌋ = VV ↔ five_rel VV.
+Theorem five__five_rel' (VV : MyNat_u): ⌊ five -⌋ = VV ↔ five_rel VV.
 Proof.
   intros. refine (five__five_rel VV).
 Qed.
@@ -4053,7 +4065,7 @@ Qed.
 
 #[global] Hint Rewrite six_inv_lem: f_rel_back.
 
-Theorem six_rel_ex : six_rel ⌊ six ⌋.
+Theorem six_rel_ex : six_rel ⌊ six -⌋.
 Proof.
   Opaque six.
   existence_lemma_pre six; fix_notations; simpl in *.
@@ -4065,7 +4077,7 @@ Qed.
 
 #[global] Opaque six.
 
-Theorem six__six_rel_rw (VV : MyNat_u): ⌊ six ⌋ = VV ↔ six_rel VV.
+Theorem six__six_rel_rw (VV : MyNat_u): ⌊ six -⌋ = VV ↔ six_rel VV.
 Proof.
   f__f_rel_rw.
 Qed.
@@ -4076,14 +4088,14 @@ Qed.
 
 #[global] Instance six_lookup_rw: dictionary rwLem six := { lookup' := six__six_rel_rw }.
 
-Theorem six__six_rel (VV : MyNat_u): ⌊ six ⌋ = VV ↔ six_rel VV.
+Theorem six__six_rel (VV : MyNat_u): ⌊ six -⌋ = VV ↔ six_rel VV.
 Proof.
   f__f_rel.
 Qed.
 
 #[global] Hint Rewrite six__six_rel: f_rel_funct_db.
 
-Theorem six__six_rel' (VV : MyNat_u): ⌊ six ⌋ = VV ↔ six_rel VV.
+Theorem six__six_rel' (VV : MyNat_u): ⌊ six -⌋ = VV ↔ six_rel VV.
 Proof.
   intros. refine (six__six_rel VV).
 Qed.
@@ -4131,7 +4143,7 @@ Qed.
 
 #[global] Hint Rewrite seven_inv_lem: f_rel_back.
 
-Theorem seven_rel_ex : seven_rel ⌊ seven ⌋.
+Theorem seven_rel_ex : seven_rel ⌊ seven -⌋.
 Proof.
   Opaque seven.
   existence_lemma_pre seven; fix_notations; simpl in *.
@@ -4143,7 +4155,7 @@ Qed.
 
 #[global] Opaque seven.
 
-Theorem seven__seven_rel_rw (VV : MyNat_u): ⌊ seven ⌋ = VV ↔ seven_rel VV.
+Theorem seven__seven_rel_rw (VV : MyNat_u): ⌊ seven -⌋ = VV ↔ seven_rel VV.
 Proof.
   f__f_rel_rw.
 Qed.
@@ -4154,14 +4166,14 @@ Qed.
 
 #[global] Instance seven_lookup_rw: dictionary rwLem seven := { lookup' := seven__seven_rel_rw }.
 
-Theorem seven__seven_rel (VV : MyNat_u): ⌊ seven ⌋ = VV ↔ seven_rel VV.
+Theorem seven__seven_rel (VV : MyNat_u): ⌊ seven -⌋ = VV ↔ seven_rel VV.
 Proof.
   f__f_rel.
 Qed.
 
 #[global] Hint Rewrite seven__seven_rel: f_rel_funct_db.
 
-Theorem seven__seven_rel' (VV : MyNat_u): ⌊ seven ⌋ = VV ↔ seven_rel VV.
+Theorem seven__seven_rel' (VV : MyNat_u): ⌊ seven -⌋ = VV ↔ seven_rel VV.
 Proof.
   intros. refine (seven__seven_rel VV).
 Qed.
@@ -4212,7 +4224,7 @@ Qed.
 
 #[global] Hint Rewrite eight_inv_lem: f_rel_back.
 
-Theorem eight_rel_ex : eight_rel ⌊ eight ⌋.
+Theorem eight_rel_ex : eight_rel ⌊ eight -⌋.
 Proof.
   Opaque eight.
   existence_lemma_pre eight; fix_notations; simpl in *.
@@ -4224,7 +4236,7 @@ Qed.
 
 #[global] Opaque eight.
 
-Theorem eight__eight_rel_rw (VV : MyNat_u): ⌊ eight ⌋ = VV ↔ eight_rel VV.
+Theorem eight__eight_rel_rw (VV : MyNat_u): ⌊ eight -⌋ = VV ↔ eight_rel VV.
 Proof.
   f__f_rel_rw.
 Qed.
@@ -4235,14 +4247,14 @@ Qed.
 
 #[global] Instance eight_lookup_rw: dictionary rwLem eight := { lookup' := eight__eight_rel_rw }.
 
-Theorem eight__eight_rel (VV : MyNat_u): ⌊ eight ⌋ = VV ↔ eight_rel VV.
+Theorem eight__eight_rel (VV : MyNat_u): ⌊ eight -⌋ = VV ↔ eight_rel VV.
 Proof.
   f__f_rel.
 Qed.
 
 #[global] Hint Rewrite eight__eight_rel: f_rel_funct_db.
 
-Theorem eight__eight_rel' (VV : MyNat_u): ⌊ eight ⌋ = VV ↔ eight_rel VV.
+Theorem eight__eight_rel' (VV : MyNat_u): ⌊ eight -⌋ = VV ↔ eight_rel VV.
 Proof.
   intros. refine (eight__eight_rel VV).
 Qed.
@@ -4293,7 +4305,7 @@ Qed.
 
 #[global] Hint Rewrite nine_inv_lem: f_rel_back.
 
-Theorem nine_rel_ex : nine_rel ⌊ nine ⌋.
+Theorem nine_rel_ex : nine_rel ⌊ nine -⌋.
 Proof.
   Opaque nine.
   existence_lemma_pre nine; fix_notations; simpl in *.
@@ -4305,7 +4317,7 @@ Qed.
 
 #[global] Opaque nine.
 
-Theorem nine__nine_rel_rw (VV : MyNat_u): ⌊ nine ⌋ = VV ↔ nine_rel VV.
+Theorem nine__nine_rel_rw (VV : MyNat_u): ⌊ nine -⌋ = VV ↔ nine_rel VV.
 Proof.
   f__f_rel_rw.
 Qed.
@@ -4316,14 +4328,14 @@ Qed.
 
 #[global] Instance nine_lookup_rw: dictionary rwLem nine := { lookup' := nine__nine_rel_rw }.
 
-Theorem nine__nine_rel (VV : MyNat_u): ⌊ nine ⌋ = VV ↔ nine_rel VV.
+Theorem nine__nine_rel (VV : MyNat_u): ⌊ nine -⌋ = VV ↔ nine_rel VV.
 Proof.
   f__f_rel.
 Qed.
 
 #[global] Hint Rewrite nine__nine_rel: f_rel_funct_db.
 
-Theorem nine__nine_rel' (VV : MyNat_u): ⌊ nine ⌋ = VV ↔ nine_rel VV.
+Theorem nine__nine_rel' (VV : MyNat_u): ⌊ nine -⌋ = VV ↔ nine_rel VV.
 Proof.
   intros. refine (nine__nine_rel VV).
 Qed.
@@ -4374,7 +4386,7 @@ Qed.
 
 #[global] Hint Rewrite ten_inv_lem: f_rel_back.
 
-Theorem ten_rel_ex : ten_rel ⌊ ten ⌋.
+Theorem ten_rel_ex : ten_rel ⌊ ten -⌋.
 Proof.
   Opaque ten.
   existence_lemma_pre ten; fix_notations; simpl in *.
@@ -4386,7 +4398,7 @@ Qed.
 
 #[global] Opaque ten.
 
-Theorem ten__ten_rel_rw (VV : MyNat_u): ⌊ ten ⌋ = VV ↔ ten_rel VV.
+Theorem ten__ten_rel_rw (VV : MyNat_u): ⌊ ten -⌋ = VV ↔ ten_rel VV.
 Proof.
   f__f_rel_rw.
 Qed.
@@ -4397,14 +4409,14 @@ Qed.
 
 #[global] Instance ten_lookup_rw: dictionary rwLem ten := { lookup' := ten__ten_rel_rw }.
 
-Theorem ten__ten_rel (VV : MyNat_u): ⌊ ten ⌋ = VV ↔ ten_rel VV.
+Theorem ten__ten_rel (VV : MyNat_u): ⌊ ten -⌋ = VV ↔ ten_rel VV.
 Proof.
   f__f_rel.
 Qed.
 
 #[global] Hint Rewrite ten__ten_rel: f_rel_funct_db.
 
-Theorem ten__ten_rel' (VV : MyNat_u): ⌊ ten ⌋ = VV ↔ ten_rel VV.
+Theorem ten__ten_rel' (VV : MyNat_u): ⌊ ten -⌋ = VV ↔ ten_rel VV.
 Proof.
   intros. refine (ten__ten_rel VV).
 Qed.
@@ -4452,7 +4464,7 @@ Qed.
 
 #[global] Hint Rewrite eleven_inv_lem: f_rel_back.
 
-Theorem eleven_rel_ex : eleven_rel ⌊ eleven ⌋.
+Theorem eleven_rel_ex : eleven_rel ⌊ eleven -⌋.
 Proof.
   Opaque eleven.
   existence_lemma_pre eleven; fix_notations; simpl in *.
@@ -4464,7 +4476,7 @@ Qed.
 
 #[global] Opaque eleven.
 
-Theorem eleven__eleven_rel_rw (VV : MyNat_u): ⌊ eleven ⌋ = VV ↔ eleven_rel VV.
+Theorem eleven__eleven_rel_rw (VV : MyNat_u): ⌊ eleven -⌋ = VV ↔ eleven_rel VV.
 Proof.
   f__f_rel_rw.
 Qed.
@@ -4476,14 +4488,14 @@ Qed.
 #[global] Instance eleven_lookup_rw: dictionary rwLem eleven := {
     lookup' := eleven__eleven_rel_rw }.
 
-Theorem eleven__eleven_rel (VV : MyNat_u): ⌊ eleven ⌋ = VV ↔ eleven_rel VV.
+Theorem eleven__eleven_rel (VV : MyNat_u): ⌊ eleven -⌋ = VV ↔ eleven_rel VV.
 Proof.
   f__f_rel.
 Qed.
 
 #[global] Hint Rewrite eleven__eleven_rel: f_rel_funct_db.
 
-Theorem eleven__eleven_rel' (VV : MyNat_u): ⌊ eleven ⌋ = VV ↔ eleven_rel VV.
+Theorem eleven__eleven_rel' (VV : MyNat_u): ⌊ eleven -⌋ = VV ↔ eleven_rel VV.
 Proof.
   intros. refine (eleven__eleven_rel VV).
 Qed.
@@ -4535,7 +4547,7 @@ Qed.
 
 #[global] Hint Rewrite twelve_inv_lem: f_rel_back.
 
-Theorem twelve_rel_ex : twelve_rel ⌊ twelve ⌋.
+Theorem twelve_rel_ex : twelve_rel ⌊ twelve -⌋.
 Proof.
   Opaque twelve.
   existence_lemma_pre twelve; fix_notations; simpl in *.
@@ -4547,7 +4559,7 @@ Qed.
 
 #[global] Opaque twelve.
 
-Theorem twelve__twelve_rel_rw (VV : MyNat_u): ⌊ twelve ⌋ = VV ↔ twelve_rel VV.
+Theorem twelve__twelve_rel_rw (VV : MyNat_u): ⌊ twelve -⌋ = VV ↔ twelve_rel VV.
 Proof.
   f__f_rel_rw.
 Qed.
@@ -4559,14 +4571,14 @@ Qed.
 #[global] Instance twelve_lookup_rw: dictionary rwLem twelve := {
     lookup' := twelve__twelve_rel_rw }.
 
-Theorem twelve__twelve_rel (VV : MyNat_u): ⌊ twelve ⌋ = VV ↔ twelve_rel VV.
+Theorem twelve__twelve_rel (VV : MyNat_u): ⌊ twelve -⌋ = VV ↔ twelve_rel VV.
 Proof.
   f__f_rel.
 Qed.
 
 #[global] Hint Rewrite twelve__twelve_rel: f_rel_funct_db.
 
-Theorem twelve__twelve_rel' (VV : MyNat_u): ⌊ twelve ⌋ = VV ↔ twelve_rel VV.
+Theorem twelve__twelve_rel' (VV : MyNat_u): ⌊ twelve -⌋ = VV ↔ twelve_rel VV.
 Proof.
   intros. refine (twelve__twelve_rel VV).
 Qed.
@@ -4744,7 +4756,7 @@ Fixpoint Modifier_wf (x : Modifier_u): Prop :=
   match x with | Minus_u => True | Natural_u => True | Plus_u => True end.
 
 Theorem Modifier_wf_ref [p : Modifier_u → Prop] (tm : {v: Modifier_u | Modifier_wf v ∧ p v}):
-  Modifier_wf ⌊ tm ⌋.
+  Modifier_wf ⌊ tm -⌋.
 Proof.
   destruct tm as [tm tm_p]. solver.
 Qed.
@@ -4794,7 +4806,7 @@ Fixpoint Letter_wf (x : Letter_u): Prop :=
   match x with | A_u => True | B_u => True | C_u => True | D_u => True | F_u => True end.
 
 Theorem Letter_wf_ref [p : Letter_u → Prop] (tm : {v: Letter_u | Letter_wf v ∧ p v}):
-  Letter_wf ⌊ tm ⌋.
+  Letter_wf ⌊ tm -⌋.
 Proof.
   destruct tm as [tm tm_p]. solver.
 Qed.
@@ -4936,7 +4948,7 @@ Qed.
 #[global] Hint Rewrite lower_letter_F_lem: f_rel_back.
 
 Theorem lower_letter_rel_ex (l : Letter_u) (l_p : Letter_wf l ∧ True):
-  lower_letter_rel l ⌊ lower_letter (exist _ l l_p) ⌋.
+  lower_letter_rel l ⌊ lower_letter (exist _ l l_p) -⌋.
 Proof.
   Opaque lower_letter.
   existence_lemma_pre lower_letter;
@@ -4952,7 +4964,7 @@ Qed.
 #[global] Opaque lower_letter.
 
 Theorem lower_letter__lower_letter_rel_rw (l : Letter_u) (l_p : Letter_wf l ∧ True) (VV : Letter_u):
-  ⌊ lower_letter (exist _ l l_p) ⌋ = VV ↔ lower_letter_rel l VV.
+  ⌊ lower_letter (exist _ l l_p) -⌋ = VV ↔ lower_letter_rel l VV.
 Proof.
   f__f_rel_rw.
 Qed.
@@ -4965,7 +4977,7 @@ Qed.
     lookup' := lower_letter__lower_letter_rel_rw }.
 
 Theorem lower_letter__lower_letter_rel (l : Letter) (VV : Letter_u):
-  ⌊ lower_letter l ⌋ = VV ↔ lower_letter_rel ⌊ l ⌋ VV.
+  ⌊ lower_letter l -⌋ = VV ↔ lower_letter_rel ⌊ l ⌋ VV.
 Proof.
   f__f_rel.
 Qed.
@@ -4973,7 +4985,7 @@ Qed.
 #[global] Hint Rewrite lower_letter__lower_letter_rel: f_rel_funct_db.
 
 Theorem lower_letter__lower_letter_rel' (l_u : Letter_u) (l : Letter) (VV : Letter_u):
-  l_u = ⌊ l ⌋ → ⌊ lower_letter l ⌋ = VV ↔ lower_letter_rel l_u VV.
+  l_u = ⌊ l ⌋ → ⌊ lower_letter l -⌋ = VV ↔ lower_letter_rel l_u VV.
 Proof.
   intros ->. refine (lower_letter__lower_letter_rel l VV).
 Qed.
@@ -5053,7 +5065,7 @@ Fixpoint Grades_wf (x : Grades_u): Prop :=
   match x with | Grade_u VV VV_ => (Letter_wf VV ∧ True) ∧ (Modifier_wf VV_ ∧ True) end.
 
 Theorem Grades_wf_ref [p : Grades_u → Prop] (tm : {v: Grades_u | Grades_wf v ∧ p v}):
-  Grades_wf ⌊ tm ⌋.
+  Grades_wf ⌊ tm -⌋.
 Proof.
   destruct tm as [tm tm_p]. solver.
 Qed.
@@ -5219,7 +5231,7 @@ Qed.
 #[global] Hint Rewrite lower_grade__Grade_F_Minus_lem: f_rel_back.
 
 Theorem lower_grade_rel_ex (g : Grades_u) (g_p : Grades_wf g ∧ True):
-  lower_grade_rel g ⌊ lower_grade (exist _ g g_p) ⌋.
+  lower_grade_rel g ⌊ lower_grade (exist _ g g_p) -⌋.
 Proof.
   Opaque lower_grade.
   existence_lemma_pre lower_grade;
@@ -5239,7 +5251,7 @@ Qed.
 #[global] Opaque lower_grade.
 
 Theorem lower_grade__lower_grade_rel_rw (g : Grades_u) (g_p : Grades_wf g ∧ True) (VV : Grades_u):
-  ⌊ lower_grade (exist _ g g_p) ⌋ = VV ↔ lower_grade_rel g VV.
+  ⌊ lower_grade (exist _ g g_p) -⌋ = VV ↔ lower_grade_rel g VV.
 Proof.
   f__f_rel_rw.
 Qed.
@@ -5252,7 +5264,7 @@ Qed.
     lookup' := lower_grade__lower_grade_rel_rw }.
 
 Theorem lower_grade__lower_grade_rel (g : Grades) (VV : Grades_u):
-  ⌊ lower_grade g ⌋ = VV ↔ lower_grade_rel ⌊ g ⌋ VV.
+  ⌊ lower_grade g -⌋ = VV ↔ lower_grade_rel ⌊ g ⌋ VV.
 Proof.
   f__f_rel.
 Qed.
@@ -5260,7 +5272,7 @@ Qed.
 #[global] Hint Rewrite lower_grade__lower_grade_rel: f_rel_funct_db.
 
 Theorem lower_grade__lower_grade_rel' (g_u : Grades_u) (g : Grades) (VV : Grades_u):
-  g_u = ⌊ g ⌋ → ⌊ lower_grade g ⌋ = VV ↔ lower_grade_rel g_u VV.
+  g_u = ⌊ g ⌋ → ⌊ lower_grade g -⌋ = VV ↔ lower_grade_rel g_u VV.
 Proof.
   intros ->. refine (lower_grade__lower_grade_rel g VV).
 Qed.
@@ -5403,7 +5415,7 @@ Theorem apply_late_policy_rel_ex
   apply_late_policy_rel
   late_days
   g
-  ⌊ apply_late_policy (exist _ late_days late_days_p) (exist _ g g_p) ⌋.
+  ⌊ apply_late_policy (exist _ late_days late_days_p) (exist _ g g_p) -⌋.
 Proof.
   Opaque apply_late_policy.
   existence_lemma_pre apply_late_policy;
@@ -5424,7 +5436,7 @@ Qed.
 
 Theorem apply_late_policy__apply_late_policy_rel_rw
   (late_days : Z) (late_days_p : True) (g : Grades_u) (g_p : Grades_wf g ∧ True) (VV : Grades_u):
-  ⌊ apply_late_policy (exist _ late_days late_days_p) (exist _ g g_p) ⌋ = VV
+  ⌊ apply_late_policy (exist _ late_days late_days_p) (exist _ g g_p) -⌋ = VV
   ↔ apply_late_policy_rel late_days g VV.
 Proof.
   f__f_rel_rw.
@@ -5439,7 +5451,7 @@ Qed.
 
 Theorem apply_late_policy__apply_late_policy_rel
   (late_days : {late_days: Z | True}) (g : Grades) (VV : Grades_u):
-  ⌊ apply_late_policy late_days g ⌋ = VV ↔ apply_late_policy_rel ⌊ late_days ⌋ ⌊ g ⌋ VV.
+  ⌊ apply_late_policy late_days g -⌋ = VV ↔ apply_late_policy_rel ⌊ late_days ⌋ ⌊ g ⌋ VV.
 Proof.
   f__f_rel.
 Qed.
@@ -5449,7 +5461,8 @@ Qed.
 Theorem apply_late_policy__apply_late_policy_rel'
   (late_days_u : Z) (g_u : Grades_u) (late_days : {late_days: Z | True}) (g : Grades) (VV : Grades_u):
   late_days_u = ⌊ late_days ⌋
-  → (g_u = ⌊ g ⌋ → ⌊ apply_late_policy late_days g ⌋ = VV ↔ apply_late_policy_rel late_days_u g_u VV).
+  → (g_u = ⌊ g ⌋
+     → ⌊ apply_late_policy late_days g -⌋ = VV ↔ apply_late_policy_rel late_days_u g_u VV).
 Proof.
   intros -> ->. refine (apply_late_policy__apply_late_policy_rel late_days g VV).
 Qed.
@@ -5612,7 +5625,7 @@ Fixpoint Day_wf (x : Day_u): Prop :=
   | Wednesday_u => True
   end.
 
-Theorem Day_wf_ref [p : Day_u → Prop] (tm : {v: Day_u | Day_wf v ∧ p v}): Day_wf ⌊ tm ⌋.
+Theorem Day_wf_ref [p : Day_u → Prop] (tm : {v: Day_u | Day_wf v ∧ p v}): Day_wf ⌊ tm -⌋.
 Proof.
   destruct tm as [tm tm_p]. solver.
 Qed.
@@ -5798,7 +5811,7 @@ Qed.
 #[global] Hint Rewrite next_weekday_Sunday_lem: f_rel_back.
 
 Theorem next_weekday_rel_ex (d : Day_u) (d_p : Day_wf d ∧ True):
-  next_weekday_rel d ⌊ next_weekday (exist _ d d_p) ⌋.
+  next_weekday_rel d ⌊ next_weekday (exist _ d d_p) -⌋.
 Proof.
   Opaque next_weekday.
   existence_lemma_pre next_weekday;
@@ -5820,7 +5833,7 @@ Qed.
 #[global] Opaque next_weekday.
 
 Theorem next_weekday__next_weekday_rel_rw (d : Day_u) (d_p : Day_wf d ∧ True) (VV : Day_u):
-  ⌊ next_weekday (exist _ d d_p) ⌋ = VV ↔ next_weekday_rel d VV.
+  ⌊ next_weekday (exist _ d d_p) -⌋ = VV ↔ next_weekday_rel d VV.
 Proof.
   f__f_rel_rw.
 Qed.
@@ -5833,7 +5846,7 @@ Qed.
     lookup' := next_weekday__next_weekday_rel_rw }.
 
 Theorem next_weekday__next_weekday_rel (d : Day) (VV : Day_u):
-  ⌊ next_weekday d ⌋ = VV ↔ next_weekday_rel ⌊ d ⌋ VV.
+  ⌊ next_weekday d -⌋ = VV ↔ next_weekday_rel ⌊ d ⌋ VV.
 Proof.
   f__f_rel.
 Qed.
@@ -5841,7 +5854,7 @@ Qed.
 #[global] Hint Rewrite next_weekday__next_weekday_rel: f_rel_funct_db.
 
 Theorem next_weekday__next_weekday_rel' (d_u : Day_u) (d : Day) (VV : Day_u):
-  d_u = ⌊ d ⌋ → ⌊ next_weekday d ⌋ = VV ↔ next_weekday_rel d_u VV.
+  d_u = ⌊ d ⌋ → ⌊ next_weekday d -⌋ = VV ↔ next_weekday_rel d_u VV.
 Proof.
   intros ->. refine (next_weekday__next_weekday_rel d VV).
 Qed.
@@ -5904,7 +5917,7 @@ Fixpoint Comparison_wf (x : Comparison_u): Prop :=
 
 Theorem Comparison_wf_ref
   [p : Comparison_u → Prop] (tm : {v: Comparison_u | Comparison_wf v ∧ p v}):
-  Comparison_wf ⌊ tm ⌋.
+  Comparison_wf ⌊ tm -⌋.
 Proof.
   destruct tm as [tm tm_p]. solver.
 Qed.
@@ -6241,7 +6254,7 @@ Qed.
 
 Theorem letter_comparison_rel_ex
   (l1 : Letter_u) (l1_p : Letter_wf l1 ∧ True) (l2 : Letter_u) (l2_p : Letter_wf l2 ∧ True):
-  letter_comparison_rel l1 l2 ⌊ letter_comparison (exist _ l1 l1_p) (exist _ l2 l2_p) ⌋.
+  letter_comparison_rel l1 l2 ⌊ letter_comparison (exist _ l1 l1_p) (exist _ l2 l2_p) -⌋.
 Proof.
   Opaque letter_comparison.
   existence_lemma_pre letter_comparison;
@@ -6271,7 +6284,7 @@ Theorem letter_comparison__letter_comparison_rel_rw
   (l2 : Letter_u)
   (l2_p : Letter_wf l2 ∧ True)
   (VV : Comparison_u):
-  ⌊ letter_comparison (exist _ l1 l1_p) (exist _ l2 l2_p) ⌋ = VV ↔ letter_comparison_rel l1 l2 VV.
+  ⌊ letter_comparison (exist _ l1 l1_p) (exist _ l2 l2_p) -⌋ = VV ↔ letter_comparison_rel l1 l2 VV.
 Proof.
   f__f_rel_rw.
 Qed.
@@ -6284,7 +6297,7 @@ Qed.
     lookup' := letter_comparison__letter_comparison_rel_rw }.
 
 Theorem letter_comparison__letter_comparison_rel (l1 l2 : Letter) (VV : Comparison_u):
-  ⌊ letter_comparison l1 l2 ⌋ = VV ↔ letter_comparison_rel ⌊ l1 ⌋ ⌊ l2 ⌋ VV.
+  ⌊ letter_comparison l1 l2 -⌋ = VV ↔ letter_comparison_rel ⌊ l1 ⌋ ⌊ l2 ⌋ VV.
 Proof.
   f__f_rel.
 Qed.
@@ -6294,7 +6307,7 @@ Qed.
 Theorem letter_comparison__letter_comparison_rel'
   (l1_u l2_u : Letter_u) (l1 l2 : Letter) (VV : Comparison_u):
   l1_u = ⌊ l1 ⌋
-  → (l2_u = ⌊ l2 ⌋ → ⌊ letter_comparison l1 l2 ⌋ = VV ↔ letter_comparison_rel l1_u l2_u VV).
+  → (l2_u = ⌊ l2 ⌋ → ⌊ letter_comparison l1 l2 -⌋ = VV ↔ letter_comparison_rel l1_u l2_u VV).
 Proof.
   intros -> ->. refine (letter_comparison__letter_comparison_rel l1 l2 VV).
 Qed.
@@ -6592,7 +6605,7 @@ Qed.
 
 Theorem modifier_comparison_rel_ex
   (m1 : Modifier_u) (m1_p : Modifier_wf m1 ∧ True) (m2 : Modifier_u) (m2_p : Modifier_wf m2 ∧ True):
-  modifier_comparison_rel m1 m2 ⌊ modifier_comparison (exist _ m1 m1_p) (exist _ m2 m2_p) ⌋.
+  modifier_comparison_rel m1 m2 ⌊ modifier_comparison (exist _ m1 m1_p) (exist _ m2 m2_p) -⌋.
 Proof.
   Opaque modifier_comparison.
   existence_lemma_pre modifier_comparison;
@@ -6618,7 +6631,8 @@ Theorem modifier_comparison__modifier_comparison_rel_rw
   (m2 : Modifier_u)
   (m2_p : Modifier_wf m2 ∧ True)
   (VV : Comparison_u):
-  ⌊ modifier_comparison (exist _ m1 m1_p) (exist _ m2 m2_p) ⌋ = VV ↔ modifier_comparison_rel m1 m2 VV.
+  ⌊ modifier_comparison (exist _ m1 m1_p) (exist _ m2 m2_p) -⌋ = VV
+  ↔ modifier_comparison_rel m1 m2 VV.
 Proof.
   f__f_rel_rw.
 Qed.
@@ -6631,7 +6645,7 @@ Qed.
     lookup' := modifier_comparison__modifier_comparison_rel_rw }.
 
 Theorem modifier_comparison__modifier_comparison_rel (m1 m2 : Modifier) (VV : Comparison_u):
-  ⌊ modifier_comparison m1 m2 ⌋ = VV ↔ modifier_comparison_rel ⌊ m1 ⌋ ⌊ m2 ⌋ VV.
+  ⌊ modifier_comparison m1 m2 -⌋ = VV ↔ modifier_comparison_rel ⌊ m1 ⌋ ⌊ m2 ⌋ VV.
 Proof.
   f__f_rel.
 Qed.
@@ -6641,7 +6655,7 @@ Qed.
 Theorem modifier_comparison__modifier_comparison_rel'
   (m1_u m2_u : Modifier_u) (m1 m2 : Modifier) (VV : Comparison_u):
   m1_u = ⌊ m1 ⌋
-  → (m2_u = ⌊ m2 ⌋ → ⌊ modifier_comparison m1 m2 ⌋ = VV ↔ modifier_comparison_rel m1_u m2_u VV).
+  → (m2_u = ⌊ m2 ⌋ → ⌊ modifier_comparison m1 m2 -⌋ = VV ↔ modifier_comparison_rel m1_u m2_u VV).
 Proof.
   intros -> ->. refine (modifier_comparison__modifier_comparison_rel m1 m2 VV).
 Qed.
@@ -6717,7 +6731,7 @@ Qed.
 Fixpoint Color_wf (x : Color_u): Prop :=
   match x with | Black_u => True | Primary_u VV => RGB_wf VV ∧ True | White_u => True end.
 
-Theorem Color_wf_ref [p : Color_u → Prop] (tm : {v: Color_u | Color_wf v ∧ p v}): Color_wf ⌊ tm ⌋.
+Theorem Color_wf_ref [p : Color_u → Prop] (tm : {v: Color_u | Color_wf v ∧ p v}): Color_wf ⌊ tm -⌋.
 Proof.
   destruct tm as [tm tm_p]. solver.
 Qed.
@@ -6843,7 +6857,7 @@ Qed.
 #[global] Hint Rewrite monochrome_Primary_lem: f_rel_back.
 
 Theorem monochrome_rel_ex (c : Color_u) (c_p : Color_wf c ∧ True):
-  monochrome_rel c ⌊ monochrome (exist _ c c_p) ⌋.
+  monochrome_rel c ⌊ monochrome (exist _ c c_p) -⌋.
 Proof.
   Opaque monochrome.
   existence_lemma_pre monochrome;
@@ -6859,7 +6873,7 @@ Qed.
 #[global] Opaque monochrome.
 
 Theorem monochrome__monochrome_rel_rw (c : Color_u) (c_p : Color_wf c ∧ True) (VV : SFBool_u):
-  ⌊ monochrome (exist _ c c_p) ⌋ = VV ↔ monochrome_rel c VV.
+  ⌊ monochrome (exist _ c c_p) -⌋ = VV ↔ monochrome_rel c VV.
 Proof.
   f__f_rel_rw.
 Qed.
@@ -6872,7 +6886,7 @@ Qed.
     lookup' := monochrome__monochrome_rel_rw }.
 
 Theorem monochrome__monochrome_rel (c : Color) (VV : SFBool_u):
-  ⌊ monochrome c ⌋ = VV ↔ monochrome_rel ⌊ c ⌋ VV.
+  ⌊ monochrome c -⌋ = VV ↔ monochrome_rel ⌊ c ⌋ VV.
 Proof.
   f__f_rel.
 Qed.
@@ -6880,7 +6894,7 @@ Qed.
 #[global] Hint Rewrite monochrome__monochrome_rel: f_rel_funct_db.
 
 Theorem monochrome__monochrome_rel' (c_u : Color_u) (c : Color) (VV : SFBool_u):
-  c_u = ⌊ c ⌋ → ⌊ monochrome c ⌋ = VV ↔ monochrome_rel c_u VV.
+  c_u = ⌊ c ⌋ → ⌊ monochrome c -⌋ = VV ↔ monochrome_rel c_u VV.
 Proof.
   intros ->. refine (monochrome__monochrome_rel c VV).
 Qed.
